commit

theories/IterativeContract.v
@@ -18,29 +18,8 @@ Inductive EventType : Type :=
 | Transfer : EventType
 | Notify : EventType.
 
+Scheme Equality for EventType.
 
-Definition eqb_event (e1 e2:EventType):bool :=
-match e1, e2 with
-| Transfer, Transfer => true
-| Notify, Notify => true
-| _, _ => false
-end.
-
-Lemma eqb_event_refl : forall (e : EventType), eqb_event e e = true.
-Proof.
-destruct e ; reflexivity.
-Qed.
-
-Lemma eqb_event_not_eq : forall (e0 e1 : EventType), e0 <> e1 -> eqb_event e0 e1 = false.
-Proof.
-destruct e0, e1;intros;try solve [contradiction | reflexivity]. 
-Qed.
-
-Definition eq_event_dec (e1 e2 : EventType) : {e1 = e2}+{~(e1=e2)}.
-Proof. destruct (eqb_event e1 e2) eqn:Heqn.
-- left. destruct e1 ; destruct e2; try reflexivity ; try discriminate Heqn.
-- right. destruct e1 ; destruct e2 ;  intro H ; try  discriminate Heqn ; try discriminate H.
-Defined.
 
 Definition Trace := List.list EventType % type.
 
@@ -52,108 +31,17 @@ Inductive Contract : Set :=
 | CSeq : Contract -> Contract -> Contract
 | Star : Contract -> Contract.
 
-
-
 Notation "e _._ c" := (CSeq (Event e) c)
-                    (at level 41, right associativity).
+                    (at level 51, right associativity).
 
 Notation "c0 _;_ c1"  := (CSeq c0 c1)
-                         (at level 50, left associativity).
+                         (at level 52, left associativity).
 
 Notation "c0 _+_ c1"  := (CPlus c0 c1)
-                         (at level 61, left associativity).
+                         (at level 53, left associativity).
 
+Scheme Equality for Contract.
 
-
-Fixpoint eqb_contract (c0 c1 : Contract) : bool :=
-match c0,c1 with
-| Success, Success => true
-| Failure, Failure => true
-| (Event e), (Event e') => eqb_event e e'
-| (CPlus c0 c1), (CPlus c2 c3) => (eqb_contract c0 c2) && (eqb_contract c1 c3)
-| (CSeq c0 c1), (CSeq c2 c3) => (eqb_contract c0 c2) && (eqb_contract c1 c3)
-| (Star c0),(Star c1) => eqb_contract c0 c1
-| _, _ => false
-end.
-
-Lemma eqb_contract_true : forall (c0 c1 : Contract), eqb_contract c0 c1 = true -> c0 = c1.
-Proof.
-induction c0. 
-- destruct c1 ; intros ; try reflexivity ; try (simpl in H ; try discriminate).
-- intros ;  destruct c1; try reflexivity; (try simpl in H ; discriminate).
-- intros. destruct c1; try reflexivity; (try simpl in H ; try discriminate).
-  apply f_equal. destruct e; destruct e0 ; try reflexivity ; try (simpl in H ; discriminate).
-- induction c1 ; intros ; try discriminate.
-  * simpl in H. apply andb_prop in H as [H1 H2].
-    apply IHc0_1 in H1. rewrite H1. apply IHc0_2 in H2.  rewrite H2.  reflexivity. 
-- induction c1 ; intros ; try discriminate. simpl in H.
-  * simpl in H. apply andb_prop in H as [H1 H2].
-    apply IHc0_1 in H1. rewrite H1. apply IHc0_2 in H2.  rewrite H2.  reflexivity.
-- induction c1 ; intros ; try discriminate. simpl in H. f_equal. auto. 
-Defined.
-
-Lemma eqb_contract_false : forall (c0 c1 : Contract), eqb_contract c0 c1 = false -> c0 <> c1.
-Proof.
-induction c0.
-- destruct c1 ; intros ; try discriminate.
-- destruct c1 ; intros ; try discriminate.
-- destruct c1 ; intros ; try discriminate.
-  * destruct e; destruct e0 ; try reflexivity ; try (simpl in H ; discriminate).
-- induction c1 ; intros ; try discriminate.
-  * simpl in H. apply andb_false_elim in H as [H1 | H1].
-    ** apply IHc0_1 in H1. intro H. inversion H. contradiction.
-    ** apply IHc0_2 in H1. intro H. inversion H. contradiction. 
-- induction c1 ; intros ; try discriminate.
-  * simpl in H. apply andb_false_elim in H as [H1 | H1].
-    ** apply IHc0_1 in H1. intro H. inversion H. contradiction.
-    ** apply IHc0_2 in H1. intro H. inversion H. contradiction.
-- induction c1 ; intros ; intro H3; try discriminate. inversion H3. simpl in H.
-  apply IHc0 in H. contradiction. 
-Defined.
-
-Definition eq_contract_dec : forall (c0 c1: Contract), {c0=c1} + {c0<>c1}.
-Proof.
-intros. destruct (eqb_contract c0 c1) eqn:Heqn.
-- left. apply eqb_contract_true. assumption.
-- right. apply eqb_contract_false. assumption.
-Defined.
-
-Lemma eq_eqb_contract_helper : forall (c : Contract), eqb_contract c c = true.
-Proof.
-induction c; try reflexivity.
-- apply eqb_event_refl.
-- simpl. rewrite IHc1. rewrite IHc2. reflexivity.
-- simpl. rewrite IHc1. rewrite IHc2. reflexivity.
-- simpl. assumption.
-Qed.
-
-Lemma eq_eqb_contract : forall (c0 c1 : Contract), c0 = c1 -> eqb_contract c0 c1 = true.
-Proof.
-intros. rewrite H. apply eq_eqb_contract_helper. 
-Qed.
-
-Lemma eqb_contract_iff : forall (c0 c1: Contract), c0 = c1 <-> eqb_contract c0 c1 = true.
-Proof.
-split. apply eq_eqb_contract. apply eqb_contract_true. Qed.
-
-Lemma neq_eqb_contract : forall (c0 c1 : Contract), c0 <> c1 -> eqb_contract c0 c1 = false.
-Proof.
-intros. destruct (eqb_contract c0 c1) eqn:Heqn. 
-- rewrite <- eqb_contract_iff in Heqn. contradiction.
-- reflexivity.
-Qed.
-
-Lemma contract_reflect : forall (c0 c1 : Contract), reflect (c0 = c1) (eqb_contract c0 c1).
-Proof.
-intros. destruct (eq_contract_dec c0 c1).
-- rewrite eq_eqb_contract. constructor; assumption. auto.
-- rewrite neq_eqb_contract. constructor; assumption. auto.
-Qed.
-
-
-
-
- 
 
 (*For a nullary contract c, nu c = true*)
 Fixpoint nu(c:Contract):bool :=
@@ -165,135 +53,64 @@ match c with
 | c0 _+_ c1 => nu c0 || nu c1
 | Star c => true
 end.
-(*
-Lemma nu_true : forall (c0 : Contract), nu c0 = true -> Nu c0.
-Proof.
-induction c0;intros;try solve [ constructor | discriminate].
-- simpl in H. apply orb_prop in H as [H | H];  auto.
-- simpl in H. apply andb_prop in H as [H1 H2];auto.
-Qed.
 
-
-Inductive NotNu : Contract -> Prop :=
-| NNFailure : NotNu Failure
-| NNEvent e : NotNu (Event e)
-| NNPLus c0 c1 (H0: NotNu c0) (H1: NotNu c1) : NotNu (c0 _+_ c1)
-| NNSeqFirst c0 c1 (H0: NotNu c0) : NotNu (c0 _;_ c1)
-| NNSeqSecond c0 c1 (H0: NotNu c1) : NotNu (c0 _;_ c1).
-Hint Constructors NotNu : core.
-
-
-Lemma nu_false : forall (c0 : Contract), nu c0 = false -> NotNu c0.
-Proof.
-induction c0;intros;try solve [ constructor | discriminate].
-- simpl in H. apply orb_false_iff in H as [H1 H2]. constructor; auto.
-- simpl in H. apply andb_false_iff in H as [H | H]. constructor;auto. apply NNSeqSecond. auto.
-Qed.
-
-
-Definition Nu_dec (c : Contract) : {Nu c}+{NotNu c}.
-Proof. destruct (nu c) eqn:Heqn.
-- left. auto using nu_true.
-- right. auto using nu_false.
-Defined.
-
-
-Lemma NotNu_negation : forall (c : Contract), NotNu c -> ~(Nu c).
-Proof.
-intros. induction H;intro H2; try solve [inversion H2 | inversion H2; contradiction]. 
-Qed.
-*)
-
+Definition o (c : Contract) := if nu c then Success else Failure.
+Hint Unfold o : core.
 
 
 (*Derivative of contract with respect to an event*)
-Equations derive(e:EventType)(c:Contract):Contract :=
-derive e Success := Failure;
-derive e Failure := Failure;
-derive e (Event e1) := if eq_event_dec e1 e then Success else Failure;
-derive e (c0 _;_ c1) := if nu c0 then ((derive e c0) _;_ c1) _+_ (derive e c1)
-                          else (derive e c0) _;_ c1;
-derive e (c0 _+_ c1) := (derive e c0) _+_ (derive e c1);
-derive e (Star c) := derive e c _;_ (Star c).
+Equations derive (c:Contract) (e:EventType) :Contract :=
+derive Success e := Failure;
+derive Failure e := Failure;
+derive (Event e') e := if (EventType_eq_dec e' e) then Success else Failure;
+derive (c0 _;_ c1) e := (derive c0 e) _;_ c1 _+_ (o c0) _;_ (derive c1 e);
+derive (c0 _+_ c1) e := (derive c0 e) _+_ (derive c1 e);
+derive (Star c) e := derive c e _;_ (Star c).
+
 Global Transparent derive.
 
-Notation "c / e" := (derive e c).
+Notation "c / e" := (derive c e)(at level 40, left associativity).
 
-(*
-Inductive Derive : Contract -> EventType -> Contract -> Prop :=
- | DSuccess e : Derive Success e Failure
- | DFailure e : Derive Failure e Failure
- | DEventS e : Derive (Event e) e Success
- | DEventF e0 e (H0: e0 <> e) : Derive (Event e0) e Failure
- | DPlus e c0 c0' c1 c1' (H0: Derive c0 e c0') (H1: Derive c1 e c1') : Derive (c0 _+_ c1) e (c0' _+_ c1')
- | DSeqNu e c0 c0' c1 c1' (H0: Nu c0) (H1: Derive c0 e c0') (H2: Derive c1 e c1'): Derive (c0 _;_ c1) e ((c0' _;_c1) _+_ c1')
- | DSeq e c0 c0' c1 (H0: NotNu c0) (H1 : Derive c0 e c0') : Derive (c0 _;_ c1) e (c0' _;_ c1)
- | DStar e c c' (H: Derive c e c') : Derive (Star c) e (c' _;_ (Star c)).
-Hint Constructors Derive : core.
+Inductive Trace_Derive : Contract -> Trace -> Contract -> Prop :=
+| Trace_Derive_Nil c : Trace_Derive c [] c
+| Trace_Derive_Cons c s c' e (H: Trace_Derive (c/e) s c') : Trace_Derive c (e::s) c'. (*rule motivated by constructor being analgous to cons on lists*)
+Hint Constructors Trace_Derive : MatchDB.
 
-Lemma Derive_derive : forall (c0 c1 : Contract)(e : EventType), Derive c0 e c1 <-> c0 / e = c1.
+Ltac autoM := auto with MatchDB.
+
+Lemma Trace_Derive_trans : forall s s' c0 c1 c2 , Trace_Derive c0 s c1 -> Trace_Derive c1 s' c2 -> Trace_Derive c0 (s++s') c2.
 Proof.
-split.
-- intros. induction H; try reflexivity. 
-  * simpl. destruct (eq_event_dec e e); try solve [ reflexivity | contradiction ].
-  * simpl. destruct (eq_event_dec e0 e); try solve [ reflexivity | contradiction ].
-  * simpl. subst. reflexivity.
-  * simpl. destruct (Nu_dec c0); subst; try reflexivity.
-    apply NotNu_negation in n. contradiction.
-  * simpl. destruct (Nu_dec c0); subst; try reflexivity.
-    apply NotNu_negation in H0. contradiction. 
-  * simpl. subst. reflexivity.
-- intros. funelim (c0 / e);simpl;auto.
-  * destruct (eq_event_dec e0 e); subst; auto.
-  * destruct (Nu_dec c1);auto. 
+intros. induction H;simpl;autoM.
 Qed.
 
-Lemma Derive_derive2 : forall (c : Contract)(e : EventType), Derive c e (c / e).
+
+
+Equations trace_derive (c : Contract) (s : Trace) : Contract :=
+trace_derive c [] := c;
+trace_derive c (e::s') := trace_derive (c/e) s'.
+Global Transparent trace_derive.
+
+Notation "c // s" := (trace_derive c s)(at level 42, left associativity).
+
+Lemma trace_derive_spec : forall (c c' : Contract)(s : Trace), c // s = c' <-> Trace_Derive c s c'.
 Proof.
-intros. rewrite Derive_derive. reflexivity. Qed.
-*)
-
-Equations matches (c:Contract)(s:Trace):bool :=
-matches c [] := nu c;
-matches c (e::s') := matches (c / e) s'.
-Global Transparent matches.
-
-(*Expression*)
-Notation "s =~ c" := (matches c s) (at level 63).
-
-Inductive Matches : Trace -> Contract -> Prop :=
- | BNu c (H : nu c = true) : Matches [] c
- | BDerive c e s  (H2 : Matches s (c / e)) : Matches (e::s) c.
-Hint Constructors Matches : core.
-
-
-
-
-
-Lemma Matches_reflect : forall (s : Trace)(c : Contract), reflect (Matches s c) (s =~ c).
-Proof.
-intros. funelim (s =~ c).
-- simpl. destruct (nu c) eqn:Heqn.
-  * constructor. auto. 
-  * constructor. intro H. inversion H. rewrite Heqn in H0. discriminate.
-- simpl. destruct (l =~ c / e) eqn:Heqn.
-  * constructor. inversion H. auto.
-  * constructor. intro H2. inversion H2. subst. inversion H. contradiction.
+split;intros.
+- funelim (trace_derive c s);simpl;autoM.
+- induction H;auto. 
 Qed.
 
-(** Relation between [matches] and [derive]. *)
-Theorem derive_spec : forall (e:EventType)(s:Trace)(c:Contract),
-  (e::s) =~ c  = s =~ c / e.
-Proof. intros e s c. simpl. reflexivity.
+Lemma trace_derive_spec2 : forall (c : Contract)(s : Trace), Trace_Derive c s (c // s).
+Proof.
+intros. remember (c//s). symmetry in Heqc0. now rewrite <- trace_derive_spec.
 Qed.
 
-Lemma derive_spec2: forall (e : EventType)(s : Trace)(c : Contract),
- Matches (e::s) c <-> Matches s (c / e).
-Proof. split;intros; (try inversion H) ; auto. Qed.
+
+Definition matchesb (c : Contract)(s : Trace) := nu (c//s).
+
 
 Reserved Notation "s ==~ re" (at level 63).
 
-Inductive matches_comp : Trace -> Contract -> Prop :=
+Inductive Matches_Comp : Trace -> Contract -> Prop :=
   | MSuccess : [] ==~ Success
   | MEvent x : [x] ==~ (Event x)
   | MSeq s1 c1 s2 c2
@@ -311,233 +128,162 @@ Inductive matches_comp : Trace -> Contract -> Prop :=
   | MStarSeq c s1 s2 (H1: s1 ==~ c) 
                      (H2: s2 ==~ Star c) 
               : s1 ++ s2 ==~ Star c
-  where "s ==~ c" := (matches_comp s c).
+  where "s ==~ c" := (Matches_Comp s c).
 
-Hint Constructors matches_comp : core.
+Derive Signature for Matches_Comp.
 
-Lemma simpl_Matches_nil_plus : forall c0 c1, nu c0 || nu c1 = true -> Matches [] (c0 _+_ c1).
-Proof. intros; constructor ; simpl ; intuition. Qed.
+Hint Constructors Matches_Comp : MatchDB.
 
-Lemma simpl_Matches_nil_seq : forall c0 c1, nu c0 && nu c1 = true -> Matches [] (c0 _;_ c1).
-Proof. intros; constructor ; simpl ; intuition. Qed.
+Ltac eq_event_destruct :=
+  repeat match goal with
+         | [ |- context[if EventType_eq_dec ?e ?e then _ else _] ] => destruct (EventType_eq_dec e e);try contradiction
+         | [ |- context[if EventType_eq_dec ?e ?e0 then _ else _] ] => destruct (EventType_eq_dec e e0)
+         | [ _ : context[if EventType_eq_dec ?e ?e then _ else _]  |- _ ] => destruct (EventType_eq_dec e e);try contradiction
+         | [ _ : context[if EventType_eq_dec ?e ?e0 then _ else _] |- _ ] => destruct (EventType_eq_dec e e0)
+         end.
 
+Lemma o_or : forall (c : Contract), o c = Success /\ nu c = true \/ o c = Failure /\ nu c = false.
+Proof.
+intros. unfold o. destruct (nu c) eqn:Heqn; intuition.
+Qed.
 
+Ltac destruct_ctx :=
+  repeat match goal with
+         | [ H: ?H0 /\ ?H1 |- _ ] => destruct H
+         | [ H: exists _, _  |- _ ] => destruct H
+         end.
 
-Hint Extern 1 =>
+Ltac o_destruct :=
   match goal with
-    | [ |- context[Matches [] (?c0 _+_ ?c1)]  ] => intros;  apply simpl_Matches_nil_plus ; intuition
-    | [ |- context[Matches [] (?c0 _;_ ?c1)]  ] => intros;  apply simpl_Matches_nil_seq ; intuition
-  end : Mbase. 
+         | [ |- context[(o ?c)] ] => destruct (o_or c);destruct_ctx
+         | [ _ : context[ (o ?c)] |- _ ] => destruct (o_or c);destruct_ctx
+         end.
 
-Lemma Matches_plus_l : forall (s : Trace)(c1 c2 : Contract), Matches s c1 -> Matches s (c1 _+_ c2).
-Proof. intros. generalize dependent c2. induction H;eauto with Mbase.
-Qed.
-
-
-
-Lemma Matches_plus_r : forall (s : Trace)(c1 c2 : Contract), Matches s c2 -> Matches s (c1 _+_ c2).
+Lemma seq_Success : forall c s, s ==~ Success _;_ c <-> s ==~ c.
 Proof.
-Proof. intros. generalize dependent c1. induction H;eauto with Mbase.
-Qed.
+split;intros. inversion H. inversion H3. subst. now simpl.
+rewrite <- (app_nil_l s). autoM.
+Qed. 
 
-Lemma Matches_seq : forall (s1 s2 : Trace)(c1 c2 : Contract), 
-Matches s1 c1 -> Matches s2 c2 -> Matches (s1 ++ s2) (c1 _;_ c2).
+Lemma seq_Failure : forall c s, s ==~ Failure _;_ c <-> s ==~ Failure.
 Proof.
-intros. induction H;simpl.
-- destruct H0;  auto with Mbase.
-  constructor. simpl. destruct (nu c) eqn:Heqn; try discriminate.
-  auto using Matches_plus_r.
-- rewrite derive_spec2. simpl. destruct (nu c) eqn:heqn ; auto.
-  auto using Matches_plus_l.
+split;intros. inversion H. inversion H3. inversion H.
 Qed.
 
-Lemma Matches_star : forall (s1 s2 : Trace)(c : Contract), 
-Matches s1 c -> Matches s2 (Star c) -> Matches (s1 ++ s2) (Star c).
+(*
+Lemma o_or : forall (c0 c1 : Contract)(s : Trace), s ==~ o c0 _;_ c1 -> nu c0 = true /\ s ==~ c1 \/ nu c0 = false /\ s ==~ Failure.
 Proof.
-intros. inversion H; auto.
-simpl; rewrite derive_spec2; simpl; auto using Matches_seq.
+intros. o_destruct. unfold o in H. destruct (nu c0). funelim (o c0).
+- rewrite <- Heqcall in H. rewrite seq_Success in H. now left.
+- rewrite <- Heqcall in H. rewrite seq_Failure in H. now right.
+Qed.*)
+
+Lemma derive_plus : forall (s : Trace)(c0 c1 : Contract), (c0 _+_ c1) // s = c0//s _+_ c1//s.
+Proof.
+induction s;intros;simpl;auto.
+Qed. 
+
+Lemma o_true : forall (c: Contract), nu c = true -> o c = Success.
+Proof.
+intros. o_destruct;auto with MatchDB. rewrite H in H1. discriminate. 
 Qed.
 
-Lemma nu_empty : forall (c : Contract), nu c = true <-> [] ==~ c.
+Lemma o_false : forall (c: Contract), nu c = false -> o c = Failure.
+Proof.
+intros. o_destruct. rewrite H in H1. discriminate. auto. 
+Qed.
+
+Hint Rewrite derive_plus  : MatchDB.
+
+Lemma nu_seq_derive : forall (e : EventType)(c0 c1 : Contract), 
+nu c0 = true -> nu (c1 / e) = true -> nu ((c0 _;_ c1) / e) = true.
+Proof.
+intros. simpl. rewrite orb_true_iff. right. rewrite o_true;auto.
+Qed.
+
+Lemma nu_plus : forall c0 c1, nu (c0 _+_ c1) = true <-> nu c0 = true \/ nu c1 = true.
+Proof.
+intros. simpl. now rewrite orb_true_iff.
+Qed.
+
+Lemma nu_Failure : forall (s : Trace)(c : Contract), nu ((Failure _;_ c)//s) = false.
+Proof.
+induction s;intros. now simpl. simpl. rewrite o_false;auto.
+rewrite derive_plus. simpl. now repeat rewrite IHs.
+Qed.
+
+Lemma nu_Success : forall (s : Trace)(c : Contract), nu ((Success _;_ c)//s) = nu (c//s).
+Proof.
+induction s;intros;simpl;auto. simp o. rewrite derive_plus.
+simpl. rewrite nu_Failure. simpl. now rewrite IHs.
+Qed.
+
+Hint Rewrite nu_Failure nu_Success : MatchDB.
+
+Lemma nu_seq_trace_derive : forall (s1 : Trace)(c0 c1 : Contract), 
+nu c0 = true -> nu (c1 // s1) = true -> nu ((c0 _;_ c1) // s1) = true.
+Proof.
+induction s1;intros;simpl in *. intuition.
+rewrite o_true;auto. rewrite derive_plus. simpl. autorewrite with MatchDB.
+rewrite H0. now rewrite orb_comm.
+Qed.
+
+Lemma matchesb_seq : forall (s0 s1 : Trace)(c0 c1 : Contract), nu (c0//s0) = true -> nu (c1//s1) = true -> nu ((c0 _;_c1) // (s0++s1)) = true.
+Proof.
+induction s0;intros;simpl in *.
+- rewrite nu_seq_trace_derive; auto. 
+- autorewrite with MatchDB. simpl. rewrite orb_true_iff. left.
+  rewrite IHs0;auto.
+Qed.
+
+Lemma Matches_Comp_i_matchesb : forall (c : Contract)(s : Trace), s ==~ c -> nu (c//s) = true.
+Proof.
+intros. induction H;auto.
+- simpl. eq_event_destruct. reflexivity.
+- rewrite matchesb_seq;auto.
+- autorewrite with MatchDB. simpl. intuition.
+- autorewrite with MatchDB. simpl. intuition.
+- destruct s1. now simpl. simpl. rewrite matchesb_seq;auto.
+Qed.
+
+
+Lemma Matches_Comp_nil : forall (c : Contract), nu c = true <-> [] ==~ c.
 Proof.
 split;intros.
-- induction c; simpl in H ; try discriminate; auto. apply orb_prop in H. destruct H;auto.
-  rewrite <- (app_nil_l []); auto.
-- induction c;auto; inversion H; simpl; intuition. 
+- induction c; simpl in H ; try discriminate; autoM. apply orb_prop in H. destruct H; autoM.
+  rewrite <- (app_nil_l []); autoM.
+- induction c;autoM; inversion H; simpl; intuition. 
   apply app_eq_nil in H1 as [H1 H1']. subst. intuition. 
 Qed.
 
+Lemma Matches_Comp_derive : forall (c : Contract)(e : EventType)(s : Trace), s ==~ c / e -> (e::s) ==~ c.
+Proof.
+induction c;intros; try solve [simpl in H; inversion H].
+- simpl in H. eq_event_destruct. inversion H. subst. autoM. inversion H.
+- simpl in H. inversion H; autoM. 
+- simpl in H. inversion H. inversion H2. subst. rewrite app_comm_cons. autoM.
+  subst. o_destruct.  
+  * rewrite H0 in H1. rewrite <- (app_nil_l (e::s)). constructor. now rewrite Matches_Comp_nil in H2.
+    rewrite seq_Success in H1. auto. 
+  * rewrite H0 in H1. inversion H1. inversion H6.
+- inversion H. rewrite app_comm_cons. autoM.
+Qed.
 
-(*
-Lemma Nu_empty : forall (c : Contract), Nu c <-> [] ==~ c.
+
+
+
+Lemma Matches_Comp_iff_matchesb : forall (c : Contract)(s : Trace), s ==~ c <-> matchesb c s = true.
 Proof.
 split;intros.
-- induction H;auto. rewrite <- (app_nil_l []). auto.
-- induction c;auto; inversion H;auto. apply app_eq_nil in H1 as [H1 H1']. subst. auto.
-Qed.*)
-
-
-Lemma derives_matches : forall (c : Contract)(e : EventType)(s : Trace), s ==~ c / e -> (e::s) ==~ c.
-Proof.
-induction c;intros;simpl in H; try solve [inversion H].
-- destruct (eq_event_dec e e0); inversion H. subst ; auto.
-- destruct (nu c1) eqn:Heqn;inversion H;auto.
-- destruct (nu c1) eqn:Heqn.
-  * inversion H.
-    ** inversion H2. rewrite app_comm_cons. auto.
-    ** rewrite <- (app_nil_l (e::s)). constructor; auto using nu_empty.
-       rewrite <- nu_empty. assumption.
-  * inversion H. rewrite app_comm_cons. auto.
-- inversion H. rewrite app_comm_cons. auto.
+- unfold matchesb. auto using Matches_Comp_i_matchesb.
+- generalize dependent c. induction s;intros. unfold matchesb in H.
+  simpl in H. now rewrite <- Matches_Comp_nil.
+  auto using Matches_Comp_derive.
 Qed.
-
-
-
-Lemma matches_Matches : forall (s : Trace)(c : Contract), s ==~ c <-> Matches s c.
-Proof.
-split ; intros.
-- induction H;auto.
-  * constructor. simpl. destruct (eq_event_dec x x). auto. contradiction.
-  * apply Matches_seq;auto.
-  * apply Matches_plus_l;auto.
-  * apply Matches_plus_r;auto.
-  * apply Matches_star;auto.
-- induction H.
-  * apply nu_empty;auto.
-  * apply derives_matches. assumption. 
-Qed.
-
-(*the proposition s ==~ c is reflected in the value s =~ c *)
-Lemma matches_reflect : forall (s : Trace) (c : Contract), reflect (s ==~ c) (s =~ c).
-Proof.
-intros. destruct (Matches_reflect s c).
-- constructor. apply matches_Matches. assumption.
-- constructor. intro H. rewrite <- matches_Matches in n. contradiction.
-Qed.
-
-Lemma matches_comp_iff_matches : forall (s : Trace)(c : Contract), s ==~ c <-> s =~ c = true.
-Proof.
-intros. destruct (matches_reflect s c).
-- split ; auto.
-- split; intros; try contradiction. discriminate. 
-Qed.
-
 
 
 Lemma derive_spec_comp : forall (c : Contract)(e : EventType)(s : Trace), e::s ==~ c <-> s ==~ c / e.
 Proof.
-intros. repeat rewrite matches_comp_iff_matches. simpl. reflexivity.
+intros. repeat rewrite Matches_Comp_iff_matchesb.  reflexivity.
 Qed.
-
-
-(*************************************************************************************)
-
-Lemma plus_comm : forall (c1 c2 : Contract),(forall s, s ==~ (c1 _+_ c2) <-> s ==~ (c2 _+_ c1)).
-Proof.
-split.
-- intros. inversion H ; auto. 
-- intros. inversion H ; auto.
-Qed.
-
-Lemma plus_assoc : forall (c1 c2 c3 : Contract), (forall s, s==~((c1 _+_ c2) _+_ c3) <-> s ==~ (c1 _+_ (c2 _+_ c3))).
-Proof.
-split;intros.
-- inversion H;auto.
-  inversion H2;auto.
-- inversion H;auto.
-  inversion H1;auto.
-Qed.
-
-Lemma seq_assoc : forall (c1 c2 c3 : Contract),forall s, s==~((c1 _;_ c2) _;_ c3) <-> s==~ (c1 _;_ (c2 _;_ c3)).
-Proof.
-split.
-- intro H. inversion H. inversion H3. rewrite <- app_assoc. apply MSeq.
-  * apply H8.
-  * apply MSeq.
-    ** apply H9.
-    ** apply H4.
-- intro H. inversion H. inversion H4. rewrite -> app_assoc. apply MSeq.
-  * apply MSeq.
-    ** apply H3.
-    ** apply H8.
-  * apply H9.
-Qed.
-
-Lemma plus_or : forall (s : Trace)(c1 c2 : Contract), s ==~ (c1 _+_ c2) <-> s ==~ c1 \/ s ==~c2.
-Proof. 
-split.
-- intros. repeat rewrite comp_iff_oper in *. inversion H; auto || auto.
-- intros. destruct H;auto. 
-Qed.
-
-Fixpoint plus_fold (l : list Contract) : Contract :=
-match l with
-| [] => Failure
-| c ::l => c _+_ (plus_fold l)
-end.
-
-
-Lemma plus_fold_app : forall (s:Trace)(l1 l2 : list Contract), 
-s ==~ plus_fold (l1 ++ l2) <-> s ==~ (plus_fold l1) _+_ (plus_fold l2).
-Proof.
-intro. induction l1.
-- intros. split.
-  * intros. simpl in H. auto.
-  * intros. simpl. simpl in H. inversion H. {  inversion H2. } assumption.
-- intros. split.
-  * intros. simpl in *. apply plus_or in H as [H | H] ; auto.
-    specialize IHl1 with l2. apply IHl1 in H. apply plus_assoc. auto.
-  * intros. simpl in *. apply plus_assoc in H. apply plus_or in H as [H | H].
-    ** auto.
-    ** apply MPlusR. apply IHl1. assumption.
-Qed.
-
-
-Lemma in_plus_fold : forall (s : Trace)(l : list Contract), s ==~ plus_fold l <-> 
-(exists c, In c l /\ s ==~ c).
-Proof.
-intros. split.
-- induction l.
-  * intros. simpl in H. inversion H.
-  * intros. simpl in H. apply plus_or in H as [H | H].
-    ** exists a. split. apply in_eq. assumption.
-    ** apply IHl in H as [c' [P1 P2]]. exists c'. split ; auto using  in_cons.
-- intros. destruct H as [ c' [P1 P2]]. induction l.
-  * destruct P1.
-  * apply in_inv in P1 as [P1 | P1].
-    ** simpl. rewrite P1. auto.
-    ** simpl. auto.
-Qed.
-
-
-
-
-
-
-Fixpoint seq_fold (l : list Contract) :=
-match l with
-| [] => Success
-| a::l' => a _;_ (seq_fold l')
-end.
-
-
-
-Lemma seq_fold_map : forall (s:Trace), s ==~ seq_fold (map Event s).
-Proof.
-induction s.
-- simpl. auto.
-- simpl. assert (HA: a::s = [a]++s). { reflexivity. } rewrite HA. constructor; auto.
-Qed.
-
-
-Lemma seq_fold_app : forall (s:Trace)(s0 s1 : list Contract), s ==~ seq_fold (s0 ++ s1) <-> s ==~ (seq_fold s0) _;_ (seq_fold s1).
-Proof.
-intros. generalize dependent s. generalize dependent s1.
-induction s0;intros.
-- simpl. split. intro. rewrite <- (app_nil_l s). constructor;auto. intros. inversion H. inversion H3. subst. simpl. assumption.
-- simpl. split.
-  * intros. inversion H. subst. rewrite seq_assoc. constructor. assumption. apply IHs0. assumption.
-  * intros. rewrite seq_assoc in H. inversion H. subst. constructor. assumption. apply IHs0. assumption.
-Qed.
-
 
