theories/IterativeEquations.v
@@ -5,6 +5,7 @@ Require Import Bool.Bool  Bool.Sumbool.
 Require Import Lists.List.
 Import ListNotations.
 Require Import Bool.Bool.
+Require Import micromega.Lia.
 From Equations Require Import Equations.
 (*******************************************************************************************************)
 Set Implicit Arguments.
@@ -101,7 +102,7 @@ Proof.
 split.
 - exists Failure. exists Failure. reflexivity.
 - split.
-  * apply eq_true_iff_eq. now repeat rewrite nu_empty.
+  * apply eq_true_iff_eq. now repeat rewrite Matches_Comp_nil.
   * intros. now repeat rewrite <- derive_spec_comp. 
 Qed.
 
@@ -112,13 +113,13 @@ split.
 - generalize dependent c1. generalize dependent c0. cofix matches_eq_is_bisimilarity.
   intros. constructor.
   * intros. apply matches_eq_is_bisimilarity. setoid_rewrite <- derive_spec_comp. auto.
-  * apply eq_true_iff_eq. repeat rewrite nu_empty. auto.
+  * apply eq_true_iff_eq. repeat rewrite Matches_Comp_nil. auto.
 - intro.
   repeat setoid_rewrite matches_Matches. intro. generalize dependent c1.
   generalize dependent c0. induction s;intros.
-  * inversion H. repeat rewrite <- matches_Matches. repeat rewrite <- nu_empty.
+  * inversion H. repeat rewrite <- matches_Matches. repeat rewrite <- Matches_Comp_nil.
     now rewrite H1.
-  * repeat rewrite derive_spec2. inversion H. auto.
+  * repeat rewrite derive_spec_comp. inversion H. auto.
 Qed.
 
 
@@ -130,8 +131,29 @@ Inductive c_eq_aci : Contract -> Contract -> Prop :=
     | cc_trans c0 c1 c2 (H1 : c0 =ACI= c1) (H2 : c1 =ACI= c2) : c0 =ACI= c2 (*transitivity*)
     | cc_ctx_plus c0 c0' c1 c1' (H1 : c0 =ACI= c0') (H2 : c1 =ACI= c1') : c0 _+_ c1 =ACI= c0' _+_ c1' (*ctx rules*)
     | cc_ctx_seq c0 c0' c1 c1' (H1 : c0 =ACI= c0') (H2 : c1 =ACI= c1') : c0 _;_ c1 =ACI= c0' _;_ c1'
-    where "c0 =ACI= c1" := (c_eq_aci c0 c1). (*skip last three rules*)
+    | cc_refl c : c =ACI= c
+    | cc_sym c0 c1 (H : c0 =ACI= c1) : c1 =ACI= c0
+    where "c0 =ACI= c1" := (c_eq_aci c0 c1).
 Hint Constructors c_eq_aci : core.
+
+Add Parametric Relation : Contract c_eq_aci
+  reflexivity proved by cc_refl
+  symmetry proved by cc_sym
+  transitivity proved by cc_trans
+  as Contract_setoid.
+
+Add Parametric Morphism : CPlus with
+signature c_eq_aci ==> c_eq_aci ==> c_eq_aci as c_eq_aci_plus_morphism.
+Proof.
+  intros. auto.
+Qed.
+
+Add Parametric Morphism : CSeq with
+signature c_eq_aci ==> c_eq_aci ==> c_eq_aci as c_eq_aci_seq_morphism.
+Proof.
+  intros. auto.
+Qed.
+
 
 Lemma c_eq_aci_nu : forall c0 c1, c0 =ACI= c1 -> nu c0 = nu c1.
 Proof.
@@ -139,6 +161,7 @@ intros. induction H;simpl; try btauto.
 - rewrite IHc_eq_aci1. auto.
 - rewrite IHc_eq_aci1. now rewrite IHc_eq_aci2. 
 - rewrite IHc_eq_aci1. now rewrite IHc_eq_aci2.
+- intuition. 
 Qed. 
 
 Ltac nu_destruct :=
@@ -146,12 +169,19 @@ Ltac nu_destruct :=
          | [ |- context[if nu ?c then _ else _] ] => destruct (nu c) eqn:?Heqn
          end.
 
+Lemma o_aci : forall c0 c1, c0 =ACI= c1 -> o c0 = o c1.
+Proof.
+intros. apply c_eq_aci_nu in H. o_destruct; unfold o; now rewrite H.
+Qed. 
+
+
 Lemma c_eq_aci_derive : forall c0 c1, c0 =ACI= c1 -> (forall e, c0/e =ACI= c1/e).
 Proof.
 intros. induction H; try solve [simpl ; eauto].
-simpl. nu_destruct;auto.
-all: apply c_eq_aci_nu in H; rewrite Heqn in H; rewrite Heqn0 in H; discriminate.
+simpl. apply cc_ctx_plus;auto. apply cc_ctx_seq;auto. nu_destruct;auto.
+apply o_aci in H. now rewrite H.
 Qed.
+
 
 Reserved Notation "c0 =R= c1" (at level 63).
 CoInductive c_eq : Contract -> Contract -> Prop :=
@@ -197,45 +227,52 @@ intros. pose proof c_eq_is_bisimilarity. pose proof matches_eq_is_bisimilarity.
 unfold bisimilarity in *. rewrite H0. now rewrite <- H1.
 Qed.
 
-(**********Decision procedure ******)
-
-Fixpoint trace_derive (c: Contract) (s : Trace) :=
-match s with
-| [] => c
-| e::s' => trace_derive (c/e) s'
-end.
-
-Lemma finitely_many_derivatives : forall c, exists (l : list Contract), (forall s, In (trace_derive c s) l).
-Proof. Admitted.
-
-Definition is_finite_bisimulation (l : list (Contract * Contract)) := 
- forall c0 c1, In (c0,c1) l -> nu c0 = nu c1 /\ 
-                     forall (e : EventType), In (c0/e, c1/e) l.
-
-(*Decision procedure: 
-  to decide c0 = c1,
-  - compute list l, satisfying is_finite_bisimulation with respect to c0 and c1
-  - test (c0,c1) is present in the list
- *)
-
-(*Showing bisimularity reduces to building a finite bisimulation list
-  and testing for membership*)
-Lemma in_finite_bisimulation_i_Bisimilarity : 
- forall (l : list (Contract*Contract)) (c0 c1 : Contract), 
- is_finite_bisimulation l -> In (c0,c1) l -> Bisimilarity c0 c1.
+Lemma c_eq_refl : forall c, c =R= c.
 Proof.
-cofix H.
-intros. constructor.
-- intro. apply H with l; auto. apply H0 in H1 as [_ H2];auto.
-- apply H0 in H1 as [H2 _];auto.
+intros. apply c_eq_completeness. split;auto.
 Qed.
 
-Definition alphabet := [Notify;Transfer].
-Global Opaque alphabet.
-Definition direct_derivatives (c : Contract) : list Contract := map (fun e => c/e) alphabet.
-Check fold_left.
-Check filter.
+Hint Immediate c_eq_refl : core.
 
+Lemma c_eq_sym : forall c0 c1, c0 =R= c1 -> c1 =R= c0.
+Proof.
+intros. apply c_eq_completeness. intros. apply c_eq_soundness with (s:=s) in H.
+now symmetry in H.
+Qed.
+
+Lemma c_eq_trans : forall c0 c1 c2, c0 =R= c1 -> c1 =R= c2 -> c0 =R= c2.
+Proof.
+intros. apply c_eq_completeness. intros. apply c_eq_soundness with (s:=s ) in H.
+apply c_eq_soundness with (s:=s ) in H0. rewrite H. now rewrite H0.
+Qed.
+
+Add Parametric Relation : Contract c_eq
+  reflexivity proved by c_eq_refl
+  symmetry proved by c_eq_sym
+  transitivity proved by c_eq_trans
+  as Contract_c_eq_setoid.
+
+Add Parametric Morphism : CPlus with
+signature c_eq ==> c_eq ==> c_eq as c_eq_plus_morphism.
+Proof.
+  intros. apply c_eq_completeness. intros. apply c_eq_soundness with (s:=s) in H. 
+   apply c_eq_soundness with (s:=s) in H0. split;intros.
+  - inversion H1;auto. apply MPlusL. now rewrite <- H. apply MPlusR. now rewrite <- H0.
+  - inversion H1;auto. apply MPlusL. now rewrite H. apply MPlusR. now rewrite H0.
+Qed.
+
+Add Parametric Morphism : CSeq with
+signature c_eq ==> c_eq ==> c_eq as c_eq_seq_morphism.
+Proof.
+  intros. apply c_eq_completeness. intros. split;intros. inversion H1. apply c_eq_soundness with (s:=s1) in H as H'.
+  constructor. now rewrite <- H'. apply c_eq_soundness with (s:=s2) in H0 as H''. now rewrite <- H''.
+  inversion H1. apply c_eq_soundness with (s:=s1) in H as H'. 
+    constructor. now rewrite H'. apply c_eq_soundness with (s:=s2) in H0 as H''. now rewrite H''.
+Qed.
+
+
+
+(*********************************************Decision procedure *****************************************)
 Section member.
   Variable A : Set.
   Hypothesis equals : A -> A -> bool.
@@ -248,17 +285,17 @@ Section member.
 End member.
 
 Definition inclb (l0 l1 : list Contract) :bool := 
- forallb (fun c0 => existsb (fun c1 => if eq_contract_dec c0 c1 then true else false) l1) l0.
+ forallb (fun c0 => existsb (fun c1 => if Contract_eq_dec c0 c1 then true else false) l1) l0.
 
 Lemma inclb_iff : forall (l0 l1 : list Contract), inclb l0 l1 = true <-> incl l0 l1.
 Proof. unfold inclb. unfold incl. split. 
 - intros. rewrite forallb_forall in H. apply H in H0. rewrite existsb_exists in H0. destruct H0 as [x [P0 P1]].
-destruct (eq_contract_dec a x).
+destruct (Contract_eq_dec a x).
   * subst. assumption.
   * discriminate.
 - intros. rewrite forallb_forall. intros. apply H in H0. rewrite existsb_exists. exists x. split.
   * assumption.
-  * destruct (eq_contract_dec x x).
+  * destruct (Contract_eq_dec x x).
     ** reflexivity.
     ** contradiction. 
 Qed.
@@ -271,6 +308,7 @@ intros. destruct (inclb l0 l1) eqn:Heqn.
 - constructor. intro H. rewrite <- inclb_iff in H. rewrite Heqn in H. discriminate.
 Qed.
 
+(*
 Fixpoint flatten_contract (c : Contract) : list Contract :=
 match c with
 | c0 _+_ c1 => (flatten_contract c0) ++ (flatten_contract c1)
@@ -285,18 +323,1238 @@ Definition aci_eq (c0 c1 : Contract) : bool :=
 Definition aci_p_eq (p0 p1: (Contract * Contract)) : bool :=
  let (c0,c0') := p0 in
  let (c1,c1') := p1 in
- aci_eq c0 c1 && aci_eq c0' c1'.
+ aci_eq c0 c1 && aci_eq c0' c1'.*)
 
+(*
+Fixpoint trace_derive (c: Contract) (s : Trace) :=
+match s with
+| [] => c
+| e::s' => trace_derive (c/e) s'
+end.*)
+
+Equations trace_derive (c : Contract) (s : Trace) : Contract :=
+trace_derive c [] := c;
+trace_derive c (e::s') := trace_derive (c/e) s'.
+Global Transparent trace_derive.
+Definition contains_all_derivatives_of c (l : list Contract) := forall (s : Trace), In (trace_derive c s) l.
+
+
+
+Inductive Trace_Derive : Contract -> Trace -> Contract -> Prop :=
+| Trace_Derive_Nil c : Trace_Derive c [] c
+| Trace_Derive_Cons c s c' e (H: Trace_Derive (c/e) s c') : Trace_Derive c (e::s) c'. (*rule motivated by constructor being analgous to cons on lists*)
+Hint Constructors Trace_Derive : core.
+
+(*
+Inductive Trace_Derive : Contract -> Trace -> Contract -> Prop :=
+| Trace_Derive_Nil c : Trace_Derive c [] c
+| Trace_Derive_Cons c s c' e (H: Trace_Derive c s c') : Trace_Derive c (s++[e]) (c'/e).
+Hint Constructors Trace_Derive : core.*)
+
+
+
+Lemma derive_trace_derive : forall (c : Contract)(s : Trace)(e :EventType), trace_derive c (s++[e]) = (trace_derive c s) / e.
+Proof.
+intros. generalize dependent c. induction s;simpl;auto.
+Qed.
+
+Lemma length_removelast : forall (A: Type)(e:A)(l:list A), length (removelast (e :: l)) = length l.
+Proof.
+intros. simpl. generalize dependent e. induction l;intros;auto. simpl. f_equal. now simpl.
+Qed.
+(*
+Lemma removelast_cons :  forall (A: Type)(e:A)(l:list A), removelast (e::l) = e::(removelast l).
+Proof.
+intros. induction l. simpl. (removelast (e :: l)) = length l.
+*)
+
+Lemma app_nil : forall (A:Type)(l:list A)(e: A), l ++ [e] = [] -> False.
+Proof.
+intros. destruct l; discriminate. 
+Qed.
+
+Lemma app_singleton : forall (A:Type)(l:list A)(e e': A), l ++ [e] = [e'] -> l = [] /\ e = e'.
+Proof.
+intro. destruct l;intros. simpl in H. injection H. auto. simpl in H.
+inversion H. apply app_nil in H2. destruct H2.
+Qed.
+
+(*
+Ltac inversion_TD_nil H :=  inversion H; try 
+                         (match goal with
+                        | [ H' : ?l ++ [?e] = [] |- _ ] => try solve [apply app_nil in H'; contradiction]
+
+                         end);subst.*)
+
+(*
+Lemma Trace_Derive_rev : forall (l:Trace)(c c' : Contract)(e: EventType), 
+Trace_Derive c (l++[e]) (c'/e) -> Trace_Derive c l c'.
+Proof.
+induction l;intros.
+- inversion_TD_nil H. subst. apply app_singleton in H0. subst.
+*)
+(*
+Lemma Trace_Derive_cons : forall (l:Trace)(c c' : Contract)(e: EventType), 
+Trace_Derive (c/e) l c' -> Trace_Derive c (e::l) c'.
+Proof.
+induction l;intros.
+inversion_TD_nil H. subst. rewrite <- (app_nil_l [e]). auto.
+
+ 2: { inversion_TD_nil.
+inversion_TD_nil H. 2: { 
+inversion H. 2: { apply app_nil in H0. contradiction. 
+intros.*)
+
+Lemma Trace_Derive_trans : forall s s' c0 c1 c2 , Trace_Derive c0 s c1 -> Trace_Derive c1 s' c2 -> Trace_Derive c0 (s++s') c2.
+Proof.
+intros. induction H;simpl;auto.
+Qed.
+
+(*
+Lemma Trace_Derive_first_der : forall (s:Trace) c0 c1 (e:EventType), Trace_Derive c0 (e :: s) c1 -> Trace_Derive (c0/e) s c1.
+Proof.
+induction s;intros.
+inversion_TD_nil H. apply app_singleton in H0. destruct H0. rewrite H1.
+rewrite H0 in H2. now inversion_TD_nil H2.
+
+ subst.
+intros. remember (e::s). induction H. discriminate.
+
+-*)
+
+
+
+Lemma trace_derive_spec : forall (c c' : Contract)(s : Trace), (trace_derive c s) = c' <-> Trace_Derive c s c'.
+Proof.
+split;intros.
+- funelim (trace_derive c s);simpl;auto.
+- induction H;auto. 
+Qed.
+
+
+
+
+
+
+(*
+Lemma max_derivative_count_non_zero : forall (c : Contract), 0 < max_derivative_count c.
+Proof.
+induction c;simpl;try lia. rewrite (mult_n_O 0) at 1. 
+apply PeanoNat.Nat.mul_lt_mono;auto.  
+transitivity (Nat.pow 2 0). simpl. lia. apply PeanoNat.Nat.pow_lt_mono_r;lia.
+rewrite (PeanoNat.Nat.add_lt_mono_r _ _ 1). simpl.
+assert (1 < Nat.pow 2 (max_derivative_count c)). { apply PeanoNat.Nat.pow_gt_1;lia. }
+lia.
+Qed.*)
+
+
+(*Lemma trace_derive_failure : forall (s : Trace), trace_derive Failure s = Failure.
+Proof. intros;induction s;auto. Qed.
+
+Lemma trace_derive_success : forall (s : Trace), trace_derive Success s = Success \/ trace_derive Success s = Failure.
+Proof.
+induction s.
+- simpl; left;auto.
+- simpl; right;  auto using trace_derive_failure.
+Qed.
+
+Ltac eq_event_destruct :=
+  repeat match goal with
+         | [ |- context[if eq_event_dec ?e ?e then _ else _] ] => destruct (eq_event_dec e e);try contradiction
+         | [ |- context[if eq_event_dec ?e ?e0 then _ else _] ] => destruct (eq_event_dec e e0)
+         end.
+Lemma trace_derive_event : forall (s : Trace)(e :EventType), trace_derive (Event e) s = Event e \/ trace_derive (Event e) s = Success 
+                                                             \/ trace_derive (Event e) s = Failure.
+Proof.
+destruct s;intros;simpl.
+- now left.
+- eq_event_destruct.
+  * right. auto using trace_derive_success.
+  * right. right. apply trace_derive_failure.
+Qed.
+
+
+Lemma trace_derive_plus : forall (c0 c1 : Contract)(s : Trace), trace_derive (c0 _+_ c1) s = (trace_derive c0) s _+_ (trace_derive c1) s.
+Proof.
+intros. funelim (trace_derive (c0 _+_ c1) s);  simpl ; auto.
+Qed.
+
+
+
+Hint Rewrite trace_derive_failure trace_derive_success trace_derive_event : trace_deriveDB.
+
+Ltac saia := simpl ; autorewrite with trace_deriveDB; intuition || auto.
+
+
+Lemma exists_disimilar_event : forall (e : EventType), exists e', e <> e'.
+Proof.
+intros;  destruct e;  try solve [ exists Transfer; intro H;discriminate | exists Notify; intro H;discriminate ].
+Qed.
+Search (In _).*)
+Definition alphabet := [Notify;Transfer].
+Lemma in_alphabet : forall (e : EventType), In e alphabet.
+Proof.
+intros. unfold alphabet; destruct e; auto using in_cons, in_eq. 
+Qed.
+Global Opaque alphabet.
 
 Fixpoint approx (A : Type) (n: nat) (f: A -> A) (arg: A) : A :=
 match n with
 | 0 => arg
-| S n' => approx n' f (f arg)
+| S n' => f (approx n' f arg)
 end.
+
+(*Lemma approx_spec : forall (A:Type)(P:A -> Prop)(n : nat)(f: A -> A)(arg:A), P (f arg) -> P (approx n f arg).
+Proof.
+intros. induction n.
+- simpl.*)
+
+(*
+Ltac record_destruct :=
+match goal with
+         | [ |- {| r |} => destruct R
+         end.*)
+Definition extend_traces_once (ll : list Trace) : list Trace :=
+ flat_map (fun e => map (fun l => e::l) ll) alphabet.
+
+
+
+Lemma extend_traces_once_spec : forall (s : Trace)(ll : list Trace)(e : EventType), 
+ In (e::s) (extend_traces_once ll) <-> In s ll.
+Proof.
+split;intros.
+- unfold extend_traces_once in H. rewrite in_flat_map in H. destruct_ctx.
+  rewrite in_map_iff in H0. destruct_ctx. inversion H0. now subst.
+- unfold extend_traces_once. rewrite in_flat_map. exists e.
+  split;auto using in_alphabet. rewrite in_map_iff. exists s;split;auto.
+Qed.
+
+Lemma extend_traces_once_length : forall (ll : list Trace)(n:nat),
+ Forall (fun s => length s = n) ll -> Forall (fun s => length s = S n ) (extend_traces_once ll).
+Proof.
+intros.
+inversion H.
+- unfold extend_traces_once. rewrite Forall_forall. intros. simpl in H1.
+  rewrite in_flat_map in H1. destruct H1. destruct H1. simpl in H2. inversion H2.
+- rewrite Forall_forall. intros. unfold extend_traces_once in H3.
+  rewrite in_flat_map in H3. destruct H3. destruct H3.
+  rewrite in_map_iff in H4. destruct H4. destruct H4. subst.
+  simpl. f_equal. rewrite Forall_forall in H. auto.
+Qed.
+
+Hint Rewrite extend_traces_once_spec : deriveDB.
+
+Ltac auto_rew := autorewrite with deriveDB using auto.
+
+Definition n_length_traces (n : nat) := approx n extend_traces_once [[]].
+
+Lemma n_length_traces_spec_helper : forall (s' s : Trace)(ll:list Trace), 
+ In s ll -> In (s'++s) (approx (length s') extend_traces_once ll).
+Proof.
+induction s';intros.
+- now simpl.
+- simpl. auto_rew. 
+Qed.
+
+Hint Unfold n_length_traces : core.
+
+Lemma in_n_length_traces_1 : forall (e : EventType), In [e] (n_length_traces 1).
+Proof.
+destruct e;simpl. 
+- unfold n_length_traces. simpl. unfold extend_traces_once. simpl. 
+  rewrite in_flat_map. exists Transfer. split;auto using in_alphabet,in_eq.
+- unfold n_length_traces. simpl. unfold extend_traces_once. simpl. 
+  rewrite in_flat_map. exists Notify. split;auto using in_alphabet,in_eq.
+Qed.
+
+
+(*Lemma list_length_1 : forall (A:Type)(l:list A), length l = 1 -> exists e, l = [e].
+Proof.
+intros. induction l. discriminate. simpl in H. inversion H.
+apply length_zero_iff_nil in H1. subst. now exists a.
+Qed.*)
+
+
+Lemma in_n_length_traces_inc_iff : forall (n:nat)(e : EventType)(s : Trace), In (e::s) (n_length_traces (S n)) <-> In s (n_length_traces n).
+Proof.
+induction n;split;intros.
+- unfold n_length_traces in H. simpl in H. rewrite extend_traces_once_spec in H.
+  unfold n_length_traces. now simpl.
+- simpl in H. destruct H. subst. apply in_n_length_traces_1. inversion H.
+- unfold n_length_traces in *. simpl in *. now rewrite extend_traces_once_spec in H.
+- unfold n_length_traces in *. simpl in *. now rewrite extend_traces_once_spec.
+Qed.
+
+Hint Rewrite in_n_length_traces_inc_iff : deriveDB.
+
+
+
+Lemma length_iff_length_traces : forall (n :nat)(s : Trace), In s (n_length_traces n) <-> length s = n.
+Proof.
+induction n;split;intros.
+- simpl in H. destruct H. now rewrite <- H. destruct H.
+- simpl.  apply length_zero_iff_nil in H. now left.
+- destruct s. unfold n_length_traces in H. simpl in H. unfold extend_traces_once in H.
+  rewrite in_flat_map in H. destruct_ctx. rewrite in_map_iff in H0. destruct_ctx. discriminate.
+  simpl. f_equal. rewrite <- IHn.  rewrite <- in_n_length_traces_inc_iff. eapply H.
+- destruct s. discriminate. rewrite in_n_length_traces_inc_iff.
+  rewrite IHn. simpl in H. auto.
+Qed.
+
+(*Lemma n_length_traces_length_aux : forall (n:nat)(s:Trace), In s (n_length_traces n) -> length s = n.
+Proof.
+induction n;intros.
+- simpl in H. destruct H. now subst. contradiction.
+- destruct s.  unfold n_length_traces in H. simpl in H.
+  unfold extend_traces_once in H. rewrite in_flat_map in H. 
+  destruct_ctx. rewrite in_map_iff in H0. destruct_ctx. discriminate. 
+  auto using in_n_length_traces_inc.
+in *. auto using extend_traces_once_length.
+Qed.
+
+Lemma n_length_traces_length_aux : forall (n:nat), Forall (fun s => length s = n)(n_length_traces n).
+Proof.
+induction n;intros.
+- simpl. unfold n_length_traces. simpl. constructor;auto.
+- unfold n_length_traces in *. simpl in *. auto using extend_traces_once_length.
+Qed.
+
+Lemma In_n_length_traces_iff_length : forall (n :nat)(s : Trace), In s (n_length_traces n) <-> length s = n.
+Proof.
+split;auto using length_i_In_n_length_traces.
+intros.
+
+
+
+
+Lemma n_length_traces_length : forall (s:Trace)(n:nat), In s (n_length_traces n) -> length s = n.
+Proof.
+intros. pose proof (n_length_traces_length_aux n). rewrite Forall_forall in H0. auto.
+Qed.*)
+ 
+Definition nth_derivatives (c : Contract)(n:nat) : list Contract :=  map (trace_derive c) (n_length_traces n).
+
+(*Nice symmetry in this lemma when unfolding left hand side with in_map_iff *)
+Lemma nth_derivatives_iff : forall (n : nat)(c c_der : Contract), In c_der (nth_derivatives c n) <-> exists (s : Trace), Trace_Derive c s c_der /\  length s = n.
+Proof.
+intros. unfold nth_derivatives. split;intros.
+- rewrite in_map_iff in H. destruct_ctx. exists x.
+  split. now rewrite <- trace_derive_spec. now rewrite <- length_iff_length_traces. 
+- destruct_ctx. rewrite in_map_iff. exists x.
+  split. now rewrite trace_derive_spec. now rewrite length_iff_length_traces.
+Qed.
+
+(*Ltac in_map_iff_destruct :=
+  repeat match goal with
+         | [ H: In ?c (map _ _) |- _ ] => rewrite in_map_iff in H
+         | [ H: ?H0 /\ ?H1 |- _ ] => destruct H
+         | [ H: exists _, _  |- _ ] => destruct H
+         end.*)
+(*
+Lemma Trace_Derive_In_nth_derivatives : forall (c c' : Contract)(s:Trace), Trace_Derive c s c' -> In c' (nth_derivatives c (length s)).
+Proof.
+intros. induction H.
+simpl. now left.
+unfold nth_derivatives in *. in_map_iff_destruct.
+rewrite in_map_iff. exists (e::x). split.
+now simpl.
+ 
+destruct IHTrace_Derive. 
+
+
+
+destruct IHTrace_Derive. in_map_iff_destruct IHTrace_Derive.
+auto.*)
+(*
+
+Lemma length_removelast : forall (A: Type)(e:A)(l:list A), length (removelast (e :: l)) = length l.
+Proof.
+intros. simpl. generalize dependent e. induction l;intros;auto. simpl. f_equal. now simpl.
+Qed.
+
+(*express lemma with n, so that induction can be done on n, instead of s, generalizing induction hypothesis*)
+Lemma trace_derive_Nth_Derivative_aux: forall (n:nat)(s:Trace)(c: Contract), length s = n -> Nth_Derivative c (trace_derive c s) n.
+Proof.
+induction n;intros. apply length_zero_iff_nil in H. now subst.
+rewrite app_removelast_last with (A:=EventType)(l:=s)(d:=Transfer).
+rewrite derive_trace_derive. constructor. apply IHn.
+destruct s. simpl in H. discriminate. rewrite length_removelast.  simpl in H.
+auto. intro H2. rewrite H2 in H. simpl in H. discriminate.
+Qed.
+
+Lemma trace_derive_Nth_Derivative: forall (s:Trace)(c: Contract), Nth_Derivative c (trace_derive c s) (length s).
+Proof.
+auto using trace_derive_Nth_Derivative_aux.
+Qed.
+
+
+
+Lemma nth_derivatives_spec : forall c c_der n, In c_der (nth_derivatives c n) -> Nth_Derivative c c_der n.
+Proof.
+intros. unfold nth_derivatives in H.
+in_map_iff_destruct H. rewrite <- H.
+apply n_length_traces_length in H0. rewrite <- H0. apply trace_derive_Nth_Derivative.
+Qed.*)
+
+(*
+Lemma nth_derivatives_spec : forall (c : Contract)(s:Trace), In (trace_derive c s) (nth_derivatives c (length s)).
+Proof.
+intros. generalize dependent c. induction s;intros;simpl; try now left.
+unfold nth_derivatives. rewrite in_map_iff. exists (a::s). split ; simpl;auto.
+apply n_length_traces_spec.
+Qed. *)
+Definition simple_n_derivative_closure (c : Contract)(n:nat) := flat_map (nth_derivatives c) (seq 0 (1+n)).
+
+Lemma nth_derivatives_in_closure : forall (c c_der : Contract)(n n':nat), n<=n' -> In c_der (nth_derivatives c n) -> In c_der (simple_n_derivative_closure c n').
+Proof.
+intros. unfold simple_n_derivative_closure. rewrite in_flat_map. exists n.
+split. apply in_seq. split;lia. auto.
+Qed.
+
+Lemma in_closure_nth_derivatives : forall (c c_der : Contract)(n' :nat),  In c_der (simple_n_derivative_closure c n') -> 
+       exists n, n<=n' /\ In c_der (nth_derivatives c n).
+Proof.
+intros. unfold simple_n_derivative_closure in H. rewrite in_flat_map in H.
+destruct_ctx. exists x. rewrite in_seq in H. destruct H. split;try lia;auto.
+Qed.
+
+Lemma simple_n_derivative_closure_spec : forall (c c_der : Contract)(n : nat), In c_der (simple_n_derivative_closure c n) <-> 
+exists (s : Trace), Trace_Derive c s c_der /\  length s <= n.
+Proof.
+split;intros.
+- apply in_closure_nth_derivatives in H. destruct_ctx. rewrite nth_derivatives_iff in H0.
+  destruct_ctx. exists x0. rewrite H1.  split;auto.
+- destruct_ctx. eapply nth_derivatives_in_closure;eauto.
+  rewrite nth_derivatives_iff. exists x. split;auto.
+Qed.
+
+Fixpoint In_mod_ACI (c : Contract) (l : list Contract) :=
+match l with
+| [] => False
+| c' ::l' => c' =ACI= c \/ In_mod_ACI c l'
+end.
+
+Lemma In_mod_ACI_i_In : forall (c : Contract) (l : list Contract), In_mod_ACI c l -> exists c', In c' l /\ c' =ACI= c.
+Proof.
+intros c l. generalize dependent c. induction l;intros.
+- simpl in H. inversion H.
+- simpl in H. destruct H.
+  * exists a. split;auto using in_eq.
+  * apply IHl in H. destruct H. exists x. destruct H. split;auto using in_cons.
+Qed.
+
+Lemma In_i_In_mod_ACI : forall (c : Contract) (l : list Contract), (exists c', In c' l /\ c' =ACI= c) -> In_mod_ACI c l.
+Proof.
+intros. generalize dependent c. induction l;intros.
+- destruct H. destruct H. simpl in H. inversion H.
+- simpl. destruct H. destruct H. simpl in H. inversion H.
+  * subst. now left.
+  * right. apply IHl. exists x;split;auto.
+Qed.
+
+Theorem In_mod_ACI_iff_In : forall (c : Contract) (l : list Contract), In_mod_ACI c l <-> exists c', In c' l /\ c' =ACI= c.
+Proof.
+split; auto using In_i_In_mod_ACI.
+intros. now apply In_mod_ACI_i_In.
+Qed.
+
+Theorem In_mod_ACI_cons : forall (c c' : Contract) (l : list Contract), In_mod_ACI c (c'::l) <-> c' =ACI= c \/ In_mod_ACI c l.
+Proof.
+split;intros.
+- rewrite In_mod_ACI_iff_In in H. destruct_ctx. induction H.
+  * subst. now left.
+  * right. rewrite In_mod_ACI_iff_In. exists x. split;auto.
+- destruct H.
+  * rewrite In_mod_ACI_iff_In. exists c'. split;auto using in_eq.
+  * rewrite In_mod_ACI_iff_In in *. destruct_ctx. exists x.
+    split;auto using in_cons,in_eq.
+Qed. 
+
+
+Definition ACI_preserving (f : Contract -> Contract) := forall c0 c1, c0 =ACI= c1 -> f c0 =ACI= f c1.
+
+Fixpoint max_derivative_count (c : Contract) :=
+match c with
+| Failure => 1
+| Success => 2
+| Event _ => 3
+| c0 _+_ c1 => (max_derivative_count c0)* (max_derivative_count c1)
+| c0 _;_ c1 => (max_derivative_count c0) * Nat.pow 2 (max_derivative_count c1)
+| Star c0 => (Nat.pow 2 (max_derivative_count c0)) - 1
+end.
+
+CoInductive Closure : Contract -> list Contract -> Prop :=
+| Closure_fix c l (H0: forall e, Closure (c/e) l) (H1 : exists c', c' =R= c /\ In c' l)  : Closure c l.
+
+Lemma In_Closure_i_Trace_Derive : forall (c: Contract)(l : list Contract), 
+Closure c l -> (forall (s : Trace)(c_der : Contract), Trace_Derive c s c_der -> exists c', c' =R= c_der /\ In c' l).
+Proof.
+intros. generalize dependent c. induction s;intros.
+- inversion H0. subst. inversion H. destruct_ctx. exists x;auto.
+- inversion H0. inversion H. subst. eapply IHs. eapply H6. eauto.
+Qed.
+
+Lemma Trace_Derive_i_In_Closure : forall (c: Contract)(l : list Contract), 
+(forall (s : Trace)(c_der : Contract), Trace_Derive c s c_der -> exists c', c' =R= c_der /\ In c' l) -> Closure c l.
+Proof.
+cofix H_co.
+intros. constructor.
+- intros. apply H_co. intros. eapply H. constructor. eauto.
+- eauto.
+Qed.
+
+Theorem Closure_iff : forall (c: Contract)(l : list Contract), 
+Closure c l <-> (forall (s : Trace)(c_der : Contract), Trace_Derive c s c_der -> exists c', c' =R= c_der /\ In c' l).
+Proof.
+split;intros. 
+- eapply In_Closure_i_Trace_Derive;eauto.
+- eapply Trace_Derive_i_In_Closure;eauto.
+Qed.
+
+Lemma Closure_Failure : Closure Failure [Failure].
+Proof.
+cofix IH. constructor.
+- intros. now simpl. 
+- exists Failure. split;auto using in_eq.
+Qed.
+
+Hint Resolve Closure_Failure : ClosureDB.
+
+Ltac autoC := auto with ClosureDB.
+
+Lemma Closure_cons : forall (c c_der : Contract)(l : list Contract), Closure c l -> Closure c (c_der::l).
+Proof.
+cofix IH.
+intros. constructor;inversion H;eauto. 
+simpl. destruct_ctx. exists x. split;auto. 
+Qed.
+
+Hint Resolve Closure_Failure Closure_cons in_eq in_cons in_nil : ClosureDB.
+
+Lemma Closure_Success : Closure Success [Success;Failure].
+Proof.
+cofix IH.
+constructor; simpl; auto with ClosureDB. exists Success. split; auto with ClosureDB.
+
+Qed.
+
+Hint Resolve Closure_Success : ClosureDB.
+
+Ltac eq_event_destruct :=
+  repeat match goal with
+         | [ |- context[if EventType_eq_dec ?e ?e then _ else _] ] => destruct (EventType_eq_dec e e);try contradiction
+         | [ |- context[if EventType_eq_dec ?e ?e0 then _ else _] ] => destruct (EventType_eq_dec e e0)
+         end.
+
+Lemma Closure_Event : forall (e : EventType), Closure (Event e) [Event e;Success;Failure].
+Proof.
+cofix IH.
+constructor; intros;simpl.
+- eq_event_destruct; auto with ClosureDB. 
+- exists (Event e). split;auto.
+Qed.
+
+Hint Resolve Closure_Event : ClosureDB.
+
+Definition plus_prod (l0 l1 : list Contract) := map (fun p => (fst p) _+_ (snd p)) (list_prod l0 l1).
+
+Hint Unfold plus_prod : ClosureDB.
+
+Lemma Closure_Plus : forall (c0 c1 : Contract)(l0 l1 : list Contract), Closure c0 l0 -> Closure c1 l1 -> 
+ Closure (c0 _+_ c1) (plus_prod l0 l1).
+Proof.
+cofix IH.
+intros. inversion H. inversion H0. constructor;simpl;eauto. destruct_ctx. exists (x0 _+_ x).
+split;auto. rewrite H2. now rewrite H6. 
+unfold plus_prod. rewrite in_map_iff. exists (x0,x). split;auto.
+apply in_prod;auto.
+Qed.
+
+Fixpoint flatten (c : Contract) : list Contract :=
+match c with
+| c0 _+_ c1 => (flatten c0) ++ (flatten c1)
+| _ => [c]
+end.
+
+Definition plus_combine (l0 l1 : list Contract) := map (fun p => (fst p) _+_ (snd p)) (combine l0 l1).
+
+Lemma flatten_non_empty : forall (c:Contract), exists c' l, flatten c = c'::l.
+Proof.
+induction c;intros.
+- exists Success. exists []. auto.
+- exists Failure. exists []. auto.
+- exists (Event e). exists []. auto.
+- destruct_ctx. exists x1. exists (x2 ++ (flatten c2)).
+  simpl. rewrite H0. now simpl.
+- exists (c1 _;_ c2). exists []. now simpl.
+- exists (Star c). exists []. now simpl.
+Qed.
+
+
+Lemma Trace_Derive_seq_head : forall s c0 c1, hd Failure (flatten ((c0 _;_ c1) // s)) = ((c0 // s) _;_ c1).
+Proof.
+induction s;intros. now simpl. simpl. rewrite derive_plus. simpl.
+destruct (flatten_non_empty ((c0 / a _;_ c1) // s)).
+destruct_ctx. rewrite <- IHs. rewrite H. now simpl.
+Qed. 
+
+Lemma Trace_Derive_seq_head2 : forall s c0 c1, exists l, (flatten ((c0 _;_ c1) // s)) = ((c0 // s) _;_ c1):: l.
+Proof.
+induction s;intros. exists []. now simpl. simpl. rewrite derive_plus. simpl.
+destruct (flatten_non_empty ((c0 / a _;_ c1) // s)). specialize IHs with (c0/a) c1.
+destruct_ctx. rewrite H0. exists (x1 ++ (flatten ((o c0 _;_ c1 / a) // s))).
+now simpl.
+Qed. 
+
+Lemma flatten_seq_derivative : forall c0 c1 e, flatten ((c0 _;_ c1)/ e) = [c0/e _;_ c1;o(c0)_;_(c1/e)].
+Proof.
+intros. now simpl.
+Qed.
+
+Lemma flatten_seq_trace_derive : forall s c0 c1 e, flatten ((c0 _;_ c1)// (e::s)) = flat_map (fun c => flatten (c//s)) (flatten ((c0 _;_ c1)/e)). 
+Proof.
+induction s;intros. now simpl. simpl. rewrite derive_plus. simpl.
+rewrite derive_plus. simpl. rewrite derive_plus. simpl.
+rewrite app_nil_r. auto.
+Qed.
+
+(*
+Lemma unfold_derive_o_seq : forall c0 c1 e, (o c0 _;_ c1) / e = Failure _;_ c1 _+_ (o (o c0)) _;_ c1/e.
+Proof.
+intros. simpl. o_destruct. rewrite H at 1. now simpl.
+rewrite H at 1. now simpl.
+Qed.
+
+
+Lemma test2 : forall c0 c1 e, Forall (fun c => exists c' s, c = (o c') _;_ (c1//s)) (flatten ((o c0 _;_ c1)/e)).
+Proof.
+intros. rewrite Forall_forall. intros. rewrite unfold_derive_o_seq in H. simpl in H.
+destruct H. subst. exists Failure. rewrite o_false;auto. exists []. now simpl.
+destruct H. subst. exists (o c0). exists [e]. now simpl. inversion H.
+Qed.*)
+
+Lemma o_derive : forall c e, (o c)/e = Failure.
+Proof.
+intros. o_destruct. unfold o. rewrite H0. now simpl. unfold o. rewrite H0. now simpl.
+Qed.
+
+Lemma Failure_trace_derive : forall s, Failure//s = Failure.
+Proof.
+induction s;intros;auto.
+Qed.
+
+Hint Immediate o_derive Failure_trace_derive : ClosureDB.
+
+(*
+Lemma test3 : forall s' c0 c1, Forall (fun c => exists c' s, c = (o c') _;_ (c1//s)) (flatten (((o c0) _;_ c1)//s')).
+Proof.
+induction s';intros.
+- rewrite Forall_forall. intros. simpl in H. destruct H.
+  * subst. exists c0. exists []. now simpl.
+  * inversion H.
+- rewrite Forall_forall. intros. simpl in H. rewrite derive_plus in H. simpl in H.
+  apply in_app_or in H. destruct H.
+  * specialize IHs' with Failure c1. rewrite Forall_forall in IHs'.
+    specialize IHs' with x. rewrite o_derive in H. apply IHs' in H. destruct_ctx.
+    exists x0. now exists x1.
+  * specialize IHs' with (o c0) (c1/a). rewrite Forall_forall in IHs'.
+    specialize IHs' with x. apply IHs' in H. destruct_ctx. subst.
+    exists x0. exists (a::x1). now simpl.
+Qed.*)
+
+Lemma o_or : forall (c : Contract), o c = Success \/ o c = Failure.
+Proof.
+intros. o_destruct. rewrite H. now left. rewrite H. now right.
+Qed.
+
+
+Theorem flatten_seq_derive_shape : forall s c0 c1, exists l, (flatten ((c0 _;_ c1) // s)) = ((c0 // s) _;_ c1):: l /\
+ Forall (fun c => exists c' s, c = (o c') _;_ (c1//s)) l.
+Proof.
+induction s;intros.
+- simpl. exists []. split;auto.
+- rewrite flatten_seq_trace_derive. rewrite flatten_seq_derivative. simpl.
+  rewrite app_nil_r. specialize IHs with (c0/a) c1 as IHs'.
+  specialize IHs with (o c0) (c1/a). destruct_ctx. rewrite H1. rewrite H.
+  exists (x ++ o c0 // s _;_ c1 / a :: x0). split;auto.
+  rewrite Forall_forall in *. intros. apply in_app_or in H3. destruct H3.
+  * apply H0 in H3. destruct_ctx. exists x2. now exists x3.
+  * simpl in H3. destruct H3. 
+    ** rewrite <- H3. destruct (o_or c0).
+      *** rewrite H4. destruct s.
+        **** simpl. exists Success. now exists [a].
+        **** simpl. rewrite Failure_trace_derive. exists Failure. 
+             now exists [a].
+      *** rewrite H4. rewrite Failure_trace_derive. exists Failure.
+          now exists [a].
+    ** apply H2 in H3. destruct_ctx. rewrite H3.
+       exists x2. now exists (a::x3).
+Qed.
+
+Lemma flatten_seq_derive_contains_seqs : forall s c0 c1 c_der, In c_der (flatten ((c0 _;_ c1) // s)) -> exists c0' c1', c0' _;_ c1' = c_der.
+Proof.
+induction s;intros.
+- simpl in H. destruct H;try contradiction. exists c0. now exists c1.
+- simpl in H. rewrite derive_plus in H. simpl in H. apply in_app_or in H. destruct H; now apply IHs in H.
+Qed.
+
+(*
+Theorem in_flatten_seq_o_derive : forall s c0 c1 c_der0 c_der1, In (c_der0 _;_ c_der1) (flatten (((o c0) _;_ c1) // s)) <-> 
+(c0' = Success \/ c0' = Failure) /\ (c1')
+
+ = ((o c0)//s _;_ c1) \/ (s <> [] /\ exists n, c_der = Success _;_ (c1 // (skipn n s)) \/ c_der = Failure _;_ (c1 // (skipn n s))).
+Proof.*)
+
+Lemma o_idempotent : forall (c : Contract), o (o c) = o c.
+Proof.
+intros. destruct (o_or c); rewrite H;auto. 
+Qed.
+
+Hint Immediate o_idempotent : ClosureDB.
+(*
+
+
+
+(c_der0 = (o c0) \/ (s <>[] /\ c_der0 = Failure)) /\ exists n, c_der1 = c1//(skipn n s).
+Proof.
+
+
+
+Theorem in_flatten_seq_o_derive : forall s c0 c1 c_der0 c_der1, In (c_der0 _;_ c_der1) (flatten (((o c0) _;_ c1) // s)) <-> 
+(c_der0 = (o c0) \/ (s <>[] /\ c_der0 = Failure)) /\ exists n, c_der1 = c1//(skipn n s).*)
+
+Ltac derive_plus_tac H := rewrite derive_plus in H; simpl in H; apply in_app_or in H; destruct H.
+Theorem in_flatten_seq_o_derive : forall s e c0 c1 c_der0 c_der1, In (c_der0 _;_ c_der1) (flatten (((o c0) _;_ c1) // (e::s))) <-> 
+(c_der0 = Failure /\ exists n, c_der1 = c1//(firstn n s)) \/ (c_der0 = o c0 /\ exists n, c_der1 = c1//(e::(firstn n s))).
+Proof.
+induction s;intros.
+- split;intros;simpl. destruct H;try contradiction. inversion H. subst.
+  left.  split;autoC. exists 0. now simpl. destruct H;try contradiction. 
+  inversion H. subst. right. split;autoC. exists 1. now simpl.
+  destruct H. destruct_ctx. subst. left. simpl. rewrite firstn_nil.
+  rewrite o_derive. auto.  destruct_ctx. destruct x. simpl in H0. subst. subst. right.
+  rewrite o_idempotent. 
+  auto. simpl in H0. subst. right. left. rewrite o_idempotent. auto.
+- split;intros.
+  * simpl trace_derive in H. remember (a::s). simpl in H.
+    derive_plus_tac H. rewrite Heql in H. rewrite o_derive in H.
+    assert (HA : Failure = o Failure). { auto. } rewrite HA in H.
+    apply IHs in H. destruct H.
+    ** destruct_ctx. subst. left.
+ rewrite <- Heql in H. simpl in H. fold in H. derive_plus_tac H. 
+    ** simpl in IHs. rewrite o_derive in H. assert (HA : Failure = o Failure). { auto. }
+       rewrite HA in H. setoid_rewrite o_idempotent in IHs. 
+       rewrite o_idempotent in H. apply IHs in H. destruct H.
+      *** destruct_ctx. subst. left. split;auto. destruct H. derive_plus_tac H.
+      *** simpl in IHs. rewrite derive_plus in H. simpl in H. simpl in H.
+
+
+
+ left.
+  destruct (o_or c0); intuition. now exists 0. left. symmetry. destruct_ctx.
+  destruct (o_or c0). destruct H. subst. rewrite H1. rewrite skipn_nil. auto.
+  destruct H. contradiction. destruct H. subst. rewrite skipn_nil. auto.
+  destruct H. contradiction.
+- split;intros.
+  * rewrite derive_plus in H. simpl in H. apply in_app_or in H. destruct H.
+    ** rewrite o_derive in H. assert (HA: Failure = o Failure). auto.
+       rewrite HA in H. apply IHs in H. destruct_ctx. subst. split.
+      *** destruct H.
+        **** subst. right. split. intro H3. discriminate. auto.
+        **** destruct H. subst. right. split. intro H3. discriminate. auto.
+      *** destruct H. subst. exists (S x). auto. exists (S x). auto.
+    ** apply IHs in H. destruct_ctx. subst. destruct H.
+      *** split. subst. rewrite o_idempotent. now left. split.
+ 
+
+  subst. rewrite H1. left.
+  destruct H. subst.  inversion H. now left. destruct_ctx. contradiction.
+
+Theorem in_flatten_seq_derive : forall s c0 c1 c_der0 c_der1, In (c_der0 _;_ c_der1) (flatten ((c0 _;_ c1) // s)) <-> 
+(c_der0 _;_ c_der1 = c0 // s _;_ c1) \/ ( s<> [] /\ (c_der0 = Success \/ c_der0 = Failure) /\ exists n, c_der1 = c1//(skipn n s)).
+Proof.
+intro. 
+induction s;intros;simpl.
+- split;intros. destruct H;try contradiction. inversion H. subst. now left.
+  destruct H. inversion H. now left. destruct_ctx. contradiction.
+- split;intros.
+  * rewrite derive_plus in H. simpl in H. apply in_app_or in H. destruct H.
+    ** apply IHs in H. destruct H.
+      *** now left.
+      *** destruct_ctx. destruct H0.
+        **** subst. right. split.  intro H2.  discriminate. split. now left. 
+             exists (S x). now simpl.
+        **** subst. right. split. intro H2. discriminate. split. now right.
+             exists (S x). now simpl.
+    ** apply IHs in H. destruct H.
+      *** inversion H. subst. left. simpl; left.
+ intuition;try contradiction. auto.
+ destruct H;subst.
+  exists 1. now simpl. split. destruct H. inversion H. subst.
+  destruct (o_or c0). rewrite H0. right. now left. rewrite H0. right. right. auto.
+  inversion H. inversion H. inversion H0. subst. exists 0. now simpl.
+  inversion H0. destruct_ctx. destruct H. destruct x.
+  * simpl in H0. subst. intuition. auto.
+ subst. destruct H;subst. simpl. now right. susbt. 
+ rewrite H.
+ rewrite Heqt in *. simpl in H. destruct H;try contradiction. inversion H.
+  now left. destruct H. rewrite Heqt. simpl. auto. now left.
+  destruct H. subst.  rewrite H.
+
+
+c_der = (c0//s _;_ c1) \/ (s <> [] /\ exists n, c_der = Success _;_ (c1 // (skipn n s)) \/ c_der = Failure _;_ (c1 // (skipn n s))).
+Proof.
+induction s;intros.
+- simpl. split;intros. destruct H. now left. contradiction. destruct H. now left.
+  destruct_ctx. destruct H. auto.
+- split;intros.
+  * simpl in H. rewrite derive_plus in H. simpl in H.
+    apply in_app_or in H. destruct H.
+    ** apply IHs in H. destruct H.
+      *** left. now simpl.
+      *** right. split;auto. intro H3. discriminate. destruct_ctx.
+          destruct H0.
+        **** rewrite H0. exists (S x). simpl. now left.
+        **** rewrite H0. exists (S x). simpl. now right.
+    ** apply IHs in H. destruct H.
+      *** right. split. intro H3. discriminate. rewrite H.
+          destruct (o_or c0).
+        **** rewrite H0. exists ( left;simpl;auto. auto. subst. simpl. rewrite IHs.
+   split split;intros.
+  * inversion H;try contradiction. now left.
+  * destruct H. now left. destruct H. destruct H.
+    ** simpl in H.
+
+
+ destruct s. 
+      *** simpl in H. destruct H;try contradiction.
+          right. split. intro. discriminate. rewrite <- H. exists 0.
+          destruct (o_or c0);rewrite H0; auto || auto.
+      *** rewrite flatten_seq_trace_derive in H. rewrite in_flat_map in H.
+          destruct_ctx.
+        **** inversion
+
+
+
+
+ ((c0 // s) _;_ c1):: l /\
+ Forall (fun c => exists c' s, c = (o c') _;_ (c1//s)) l.
+
+
+Check firstn.
+Inductive Flat_Seq_Derivative : Contract -> Contract -> Trace -> nat -> list Contract -> Prop :=
+| FSD_Single c0 c1 s : Flat_Seq_Derivative c0 c1 s 0 [c0//s _;_ c1]
+| FSD_Cons c0 c1 s n l (H: Flat_Seq_Derivative c0 c1 s n l) : Flat_Seq_Derivative c0 c1 s (S n) (c1//(firstn (S n) s)::l).
+
+Ltac in_forall HF HIn := rewrite Forall_forall in HF; apply HF in HIn;destruct_ctx;subst.
+
+Lemma flatten_seq_derive_FSD : forall c0 c1 c_der s l, Flat_Seq_Derivative c0 c1 s (length s) l -> 
+ In c_der (flatten ((c0 _;_ c1) // s)) <-> ((exists c', c' =R= c_der /\ In c' l) \/ c_der =R= Failure).
+Proof. 
+intros. remember (length s). induction H.
+- simpl. symmetry in Heqn. apply length_zero_iff_nil in Heqn. subst. destruct (flatten_seq_derive_shape [] c0 c1). destruct H. split;intros.
+  * rewrite H in H1. simpl in H1. destruct H1.
+    ** subst. simpl. left. exists (c0 _;_ c1). split;auto.
+    ** in_forall H0 H1. simpl. destruct (o_or x0). 
+      *** rewrite H1. left. exists (c0 _;_ c1). split. split;auto.
+
+
+
+  * inversion H1. subst. rewrite H.  auto using in_eq. contradiction.
+  * rewrite H in H1. simpl in H1. destruct H1;auto.
+    rewrite Forall_forall in H0. apply H0 in H1. destruct_ctx. subst.
+    ** now left. 
+    rewrite Forall_forall in H1.
+
+Lemma FSD_max_length : forall c0 c1 c_der s l, n > length s ->  Flat_Seq_Derivative c0 c1 s n l ...
+
+Definition seq_closure_list (c0 c1 : Contract) (l0 l1 : list Contract) := 
+ let first_elements := map (fun c => c _;_ c1) l0 in
+ let mid_success_elems := map (fun c => Success _;_ c) l1 in
+ let mid_failure_elems := map (fun c => Failure _;_ c) l1 in
+ 
+
+Lemma Closure_Seq : forall (c0 c1 : Contract)(l0 l1 : list Contract), Closure c0 l0 -> Closure c1 l1 -> 
+ Closure (c0 _;_ c1) ((map (fun c => c _;_ c1) l0) ++ ) l1).
+
+
+(*Lemma Trace_Derive_seq_tail : forall  l e s c0 c1 c', flatten ((c0 _;_ c1) // s) = e::l ->
+In c' l -> exists c'' n, Trace_Derive c1 (firstn n s) c'' /\ (c' = Success _;_ c'' \/ c' = Failure _;_ c'').
+Proof.
+induction l;intros.
+- simpl in H0. inversion H0.
+- simpl in H0. inversion H0.
+  * rewrite derive_plus in H. simpl in H.
+  destruct (flatten_non_empty ((c0 / a _;_ c1) // s)).
+  destruct_ctx. rewrite H0 in H. simpl in H. apply in_app_or in H.
+  destruct H.
+  *
+
+  destruct (flatten_non_empty ((c0 _;_ c1) // (a :: s))).
+Trace_Derive (c0 _;_ c1) s c_der -> In_mod_ACI c_der ???
+
+
+
+Definition decompose_seq_aux (c0 c1 : Contract) (s : Trace) := 
+match s with
+| [] => if nu c0 then
+ (trace_derive c0 s) _;_ c1 _+_ 
+
+
+Lemma Trace_Derive_seq : forall (c0 c1 c_der : Contract)(s : Trace), Trace_Derive (c0 _;_ c1) s c_der ->
+ c_der =ACI= *)
+
+Lemma plus_prod_length : forall (l0 l1 : list Contract), length (plus_prod l0 l1) = length l0 * length l1.
+Proof.
+intros. unfold plus_prod. rewrite map_length. now rewrite prod_length.
+Qed.
+
+Hint Resolve Closure_Plus  : ClosureDB.
+
+Lemma exists_finite_closure : forall (c : Contract), exists (l : list Contract), Closure c l /\ length l = max_derivative_count c.
+Proof.
+induction c;intros.
+- exists [Success;Failure]. split;auto with ClosureDB. 
+- exists [Failure]. split;auto with ClosureDB.
+- exists [Event e;Success;Failure]. split;auto with ClosureDB.
+- destruct_ctx. exists (plus_prod x0 x). split;simpl; auto with ClosureDB.
+  rewrite plus_prod_length. rewrite H2. now rewrite H0.
+-
+  rewrite prod_length.
+  simpl.
+
+Definition simple_derivative_closure (c : Contract) := simple_n_derivative_closure c (max_derivative_count c).
+
+
+Eval compute in flat_map (nth_derivatives Failure) (seq 0 1).
+Lemma simple_derivative_closure_spec_helper : forall (n:nat)(c : Contract)(s:Trace), length s <n -> 
+In (trace_derive c s) (flat_map (nth_derivatives c) (seq 0 n)).
+Proof.
+induction n;intros.
+- simpl. destruct s;simpl in H; inversion H.
+- rewrite in_flat_map. exists (length s). split; auto using nth_derivatives_spec.
+  rewrite in_seq. simpl.  unfold lt. split; auto.
+    transitivity (length s);lia.
+Qed.
+
+
+Lemma in_simple_derivative_closure : forall (c : Contract)(s : Trace), length s < max_derivative_count c ->
+ In (trace_derive c s) (simple_derivative_closure c).
+Proof.
+intros. unfold simple_derivative_closure. now apply simple_derivative_closure_spec_helper.
+Qed.
+
+Lemma in_simple_derivative_closure_failure_success : In Failure (simple_derivative_closure Success).
+Proof. unfold simple_derivative_closure. rewrite in_flat_map. exists 1.
+rewrite in_seq.
+split;auto. rewrite <- (trace_derive_failure [Transfer]). apply nth_derivatives_spec.
+Qed.
+
+Lemma in_simple_derivative_closure_success_event : forall (e : EventType), In Success (simple_derivative_closure (Event e)).
+Proof.
+intros.
+unfold simple_derivative_closure. rewrite in_flat_map. exists 1.
+rewrite in_seq.
+split;simpl;auto. assert (HA: Success = (trace_derive (Event e) [e])). { simpl. now eq_event_destruct. }
+rewrite HA. apply nth_derivatives_spec.
+Qed.
+
+Hint Unfold simple_derivative_closure : core.
+
+(*
+Lemma in_simple_derivative_closure_trans : forall (c0 c1 c2 : Contract), In c0 (simple_derivative_closure c1) ->
+In c1 (simple_derivative_closure c2) -> In c0 (simple_derivative_closure c2).
+Proof.
+intros. unfold simple_derivative_closure in *. rewrite in_flat_map in *.
+destruct H. destruct H0. exists (x+x0). split.
+- destruct H. destruct H0. rewrite in_seq in *. split;simpl in *. lia.*)
+
+Lemma in_simple_derivative_closure_failure_event : forall (e : EventType), In Failure (simple_derivative_closure (Event e)).
+Proof.
+intros.
+ unfold simple_derivative_closure. rewrite in_flat_map. exists 1.
+ split;simpl;auto. destruct ((exists_disimilar_event e)). 
+ assert (HA: Failure = trace_derive (Event e) [x]). { simpl. now eq_event_destruct. }
+ rewrite HA. apply nth_derivatives_spec.
+Qed.
+
+Print In.
+
+ 
+
+(*
+Lemma In_mod_ACI_iff : forall (f : Contract -> Contract) 
+         (l : list Contract) (y : Contract), ACI_preserving f ->
+       In_mod_ACI y (map f l) <->
+       (exists x : Contract, f x =ACI= y /\ In_mod_ACI x l).
+Proof.
+split;intros.
+- rewrite In_mod_ACI_iff_In in H0. destruct H0. destruct H0.
+  rewrite in_map_iff in H0. destruct H0. destruct H0. exists x0. 
+  rewrite H0. split;auto. rewrite In_mod_ACI_iff_In. exists x0. split;auto.
+- destruct H0. destruct H0. rewrite In_mod_ACI_iff_In. 
+  rewrite In_mod_ACI_iff_In in H1. destruct H1. exists (f x0). split.
+  * rewrite in_map_iff. exists x0. destruct H1. split ;auto.
+  * destruct H1. inversion H0.
+    ** rewrite H4. auto. subst. unfold ACI_preserving in H. auto.
+    **
+ f_equal. symmetry in H1. auto.
+  rewrite In_mod_ACI_iff_In in H0. destruct H0. destruct H0. exists  exists (f x).
+  split;auto. rewrite in_map_iff. 
+    split;auto. exists x.
+   rewrite in_map_iff in H. destruct H. destruct H. exists x. split;auto.
+  rewrite In_mod_ACI_iff_In. exists x. split;auto.
+- destruct H. destruct H. rewrite in_map_iff. exists x.
+intros. split;intros.*)
+
+Ltac In_mod_destruct H := rewrite In_mod_ACI_iff_In in H; destruct H; destruct H;
+rewrite in_map_iff in H; destruct H; destruct H.
+Definition simple_n_derivative_closure (c : Contract) (n:nat) := flat_map (nth_derivatives c) (seq 0 n).
+Definition plus_combine (l0 l1 : list Contract) := map (fun p => (fst p) _+_ (snd p)) (combine l0 l1).
+Lemma simple_derivative_closure_plus : forall c0 c1, simple_derivative_closure (c0 _+_ c1) =
+plus_combine (simple_n_derivative_closure c0 (max_derivative_count (c0 _+_ c1))) 
+             (simple_n_derivative_closure c1 (max_derivative_count (c0 _+_ c1))).
+Proof. Admitted.
+
+Lemma derivative_closure_in_list_prod : forall c0 c1 c_der,
+  (forall s, In_mod_ACI (trace_derive c0 s) (simple_derivative_closure c0)) -> 
+  (forall s, In_mod_ACI (trace_derive c1 s) (simple_derivative_closure c1)) -> 
+  In_mod_ACI c_der (map (fun p => (fst p) _+_ (snd p))(list_prod (simple_derivative_closure c0) (simple_derivative_closure c1)))
+ -> In_mod_ACI c_der (simple_derivative_closure (c0 _+_ c1)).
+Proof. 
+intros. rewrite simple_derivative_closure_plus. rewrite In_mod_ACI_iff_In.
+In_mod_destruct H1. destruct x0.
+rewrite in_prod_iff in H3. destruct H3.
+subst. simpl in H2. exists (c _+_ c2). subst. simpl in H2. split;auto.
+unfold simple_derivative_closure. simpl.
+-
+
+ rewrite In_mod_ACI_iff_In in H1. destruct H1. destruct H1.
+rewrite in_map_iff in H1. destruct H1. destruct H1.
+rewrite In_mod_ACI_iff_In.
+(*Lemma derivative_closure_in_list_prod : forall c0 c1 c_der, In c_der (simple_derivative_closure (c0 _+_ c1)) 
+-> In_mod_ACI c_der (map (fun p => (fst p) _+_ (snd p))(list_prod (simple_derivative_closure c0) (simple_derivative_closure c1))).
+Proof.
+intros. unfold simple_derivative_closure in H. rewrite in_flat_map in H.
+destruct H. destruct H. rewrite 
+
+Lemma simple_derivative_closure_plus : forall (c0 c1 : Contract)(s : Trace),
+ (forall s, exists c0', trace_derive c0 s =ACI= c0' /\ In c0' (simple_derivative_closure c0)) ->
+ (forall s, exists c1', trace_derive c1 s =ACI= c1' /\ In c1' (simple_derivative_closure c1)) ->
+ exists c', trace_derive (c0 _+_ c1) s =ACI= c' /\ 
+ In c' (map (fun p => (fst p) _+_ (snd p))(list_prod (simple_derivative_closure c0) (simple_derivative_closure c1))).
+Proof.
+intros.
+Admitted.*)
+(* unfold simple_derivative_closure in H1. rewrite in_flat_map in H1.
+destruct H1. destruct H1. unfold nth_derivatives in H2. rewrite in_map_iff in H2.
+destruct H2. destruct H2. rewrite trace_derive_plus in H2.
+rewrite in_map_iff. specialize H with x0. specialize H0 with x0.
+destruct H. destruct H. destruct H0. destruct H0. exists (x1, x2).
+split. injection H2. exists (trace_derive c0 x0, trace_derive c1 x0).
+split.
+- now simpl.
+- rewrite in_prod_iff. split. simpl in H. rewrite in_seq in H. destruct H.
+simpl in H2. pose proof (n_length_traces_length x). rewrite Forall_forall in H3. 
+apply H3 in H1. apply in_simple_derivative_closure. rewrite H1. Search (?a < ?b * _).
+assert (HA: x = x * 1). { lia. } rewrite HA in H2. SearchRewrite (1 * _).
+ lia. subst. unfold incl. intr*)
+
+(*To show P for derivative_closure of c0 _+_ c1, it suffices to show it for cartesian product of c0' and c1's closure*)
+
+
+(*Contracts from all ACI equivalence classes are present in the simple derivative closure *)
+Lemma simple_derivative_closure_spec : forall (c : Contract) (s : Trace), 
+In_mod_ACI (trace_derive c s) (simple_derivative_closure c).
+Proof.
+induction c;intros.
+- rewrite In_mod_ACI_iff_In. destruct (trace_derive_success s).
+  * exists Success. rewrite H. saia. 
+  * exists Failure. rewrite H. split;auto using in_simple_derivative_closure_failure_success.
+- rewrite In_mod_ACI_iff_In. exists Failure. saia.
+- rewrite In_mod_ACI_iff_In. destruct (trace_derive_event s e).
+  * exists (Event e). rewrite H. saia.
+  * destruct H.
+    ** exists Success. rewrite H. split; auto using in_simple_derivative_closure_success_event. 
+    ** exists Failure. rewrite H. split;auto using in_simple_derivative_closure_failure_event.
+- apply derivative_closure_in_list_prod;auto.
+  specialize IHc1 with s. specialize IHc2 with s. rewrite In_mod_ACI_iff_In in *.
+  destruct IHc1. destruct IHc2. exists (x _+_ x0). split.
+  * rewrite in_map_iff. exists (x, x0). split;auto.
+    destruct H. destruct H0.
+    apply in_prod;auto.
+  * rewrite trace_derive_plus. destruct H. destruct H0.
+    rewrite H1. now rewrite H2.
+-
+ Admitted. 
+
+
+
+(*All derivatives of c can be found with traces of size max_derivative_count c or less *)
+(*Remember rewrite c0 _;_ c1 / e to using the o-notation*)
+Theorem finite_distinct_derivatives : forall (c : Contract)(s : Trace), exists s', 
+ length s' < max_derivative_count c /\ (trace_derive c s) =ACI= (trace_derive c s').
+Proof with (simpl;intuition || auto). 
+induction c;intros.
+- simpl. destruct s;simpl.
+  * exists []. saia. 
+  * exists [Transfer]. saia. 
+- simpl. exists []. saia. 
+- simpl. destruct s eqn:Heqn.
+  * exists []. saia.
+  * simpl. eq_event_destruct.
+    ** destruct (trace_derive_success t);rewrite H.
+      *** exists [e]. simpl. eq_event_destruct; saia. 
+      *** destruct (exists_disimilar_event e). exists [x]. simpl.
+          eq_event_destruct. contradiction. saia.
+    ** destruct (exists_disimilar_event e). exists [x]. simpl.
+          eq_event_destruct. contradiction. saia.
+- simpl. setoid_rewrite trace_derive_plus. induction s.
+  * exists []. simpl. split;auto.
+    rewrite (mult_n_O 0) at 1. auto using PeanoNat.Nat.mul_lt_mono, max_derivative_count_non_zero.
+  *
+    ** 
+
+ exists [].
+-
+    ** exists [e]. saia.
+  simpl. intuition || auto.
+ assert (HA : exists 
+
+
+
+
+
+
+
+(*Drawback, contains duplicates*)
+Definition derivative_closure_once (l_pair : (list Contract) * (list Contract)) :=
+ let (internal_nodes,leafs) := l_pair in
+ (internal_nodes++leafs,flat_map (fun c => map (fun e => c/e) alphabet) leafs).
+
+
+
+(*include c in left list to represent value of (trace_derive c []) *)
+(*More effecient way to compute derivative closure than trivially iterating over all trace with trace_derive*)
+Definition approx_derivative_closure (n : nat) (c : Contract) :=
+ approx n derivative_closure_once ([c],[c]).
+
+Lemma trace_derive_in_derivative_closure_snd : forall (c : Contract) (s : Trace), In (trace_derive c s) (snd (approx_derivative_closure (length s) c)).
+Proof. Admitted.
+
+Lemma derivative_closure_snd_in_fst : forall n n' c c_der , In c_der (snd (approx_derivative_closure n c)) -> 
+                                                            n<n' -> In c_der (fst (approx_derivative_closure n' c)).
+Proof. Admitted.
+
+Definition derivative_closure (c : Contract) : list Contract := fst (approx_derivative_closure (max_derivative_count c) c).
+
+Lemma simple_derivative_closure_i_derivative_closure : forall c,incl (simple_derivative_closure c) (derivative_closure c).
+Proof. Admitted.
+
+Lemma derivative_closure_i_simple_derivative_closure : forall c,incl (derivative_closure c) (simple_derivative_closure c).
+Proof. Admitted.
+
+Lemma derivative_closure_spec : forall (c : Contract), contains_all_derivatives_of c (derivative_closure c).
+Proof. Admitted.
+
+
+(*********************************************Extend to pairs of contracts***************************)
+Fixpoint trace_p_derive (p: Contract * Contract) (s : Trace) :=
+match s with
+| [] => p
+| e::s' => trace_p_derive (fst p / e, snd p /e) s'
+end.
+
+
+Definition p_derivative_closure_once (l_pair : (list (Contract*Contract)) * (list (Contract * Contract))) :=
+ let (internal_nodes,leafs) := l_pair in
+ (internal_nodes++leafs,flat_map (fun p => map (fun e => ((fst p) / e,(snd p) / e)) alphabet) leafs).
+
+Definition approx_p_derivative_closure (n : nat) (p : (Contract * Contract)) :=
+ approx n p_derivative_closure_once ([p],[p]).
+
+Lemma trace_derive_in_p_derivative_closure_snd : forall (c0 c1: Contract) (s : Trace), In (trace_p_derive (c0,c1) s) (snd (approx_p_derivative_closure (length s) (c0,c1))).
+Proof. Admitted.
+
+Lemma p_derivative_closure_snd_in_fst : forall n n' p p_der , In p_der (snd (approx_p_derivative_closure n p)) -> 
+                                                            n<n' -> In p_der (fst (approx_p_derivative_closure n' p)).
+Proof. Admitted.
+
+Definition max_p_derivative_count (p : Contract * Contract) := (max_derivative_count (fst p)) * (max_derivative_count (snd p)).
+
+Definition all_p_derivatives (p : Contract * Contract) : list (Contract * Contract) := fst (approx_p_derivative_closure (max_p_derivative_count p) p).
+
+Lemma all_p_derivatives_spec : forall (c0 c1 : Contract)(s : Trace), In (trace_p_derive (c0,c1) s) (all_p_derivatives (c0,c1)).
+Proof. Admitted.
+
+
+(*Show lemma that all derivatives are in derivative_closure*)
+Lemma derivative_closure_is_bisimulation : forall (c0 c1 : Contract), 
+ Forall (fun (p : Contract * Contract) => nu (fst p) = nu (snd p)) (all_p_derivatives (c0,c1)) -> bisimulation (fun x y => (In (x,y) (all_p_derivatives (c0,c1)))).
+Proof. Admitted.
+
+Definition decide_contract_equivalence (c0 c1 : Contract) := 
+ forallb (fun (p : Contract * Contract) => eqb (nu (fst p)) (nu (snd p))) (all_p_derivatives (c0,c1)).
+
+
+Lemma Bisimilarity_reflect : forall (c0 c1 : Contract), reflect (Bisimilarity c0 c1) (decide_contract_equivalence c0 c1).
+Proof. Admitted.
+
+
+
+
+
+
+
+
+
+
+
+
+
+
+
+
+
+
+
+
+
+
+
+
+
+
+
+
+
+
+
+
+
+
+
+
+
+
+
+(*Maybe keep*)
+Lemma finitely_many_derivatives : forall c, exists (l : list Contract), (forall s, member aci_eq (trace_derive c s) l = true).
+Proof. Admitted.
+
+
+Global Opaque alphabet.
+Definition direct_derivatives (c : Contract) : list Contract := map (fun e => c/e) alphabet.
+
+
+
+
+
 
 Definition direct_p_derivatives (p : Contract * Contract) : list (Contract * Contract) := 
  map (fun e => ((fst p) / e,(snd p) / e)) alphabet.
-
+(*processed contract -> all direct derivatives are in either internal_nodes or leafs
+  not processed contract -> no direct derivatives in either internal_nodes or leafs*)
 Definition p_derivative_closure_once (l_pair : (list (Contract*Contract)) * (list (Contract * Contract))) :=
  let (internal_nodes,leafs) := l_pair in
  let internal_nodes' := internal_nodes++leafs in
@@ -306,6 +1564,11 @@ Definition p_derivative_closure_once (l_pair : (list (Contract*Contract)) * (lis
 Definition approx_p_derivative_closure (n : nat) (p : (Contract * Contract)) :=
  approx n p_derivative_closure_once ([],[p]).
 
+
+(*All internal_nodes and leafs share the property that they can be derived from trace_derive c s
+  with some trace s. Only new derivatives are placed in leafs, and finitely_many_derivatives states
+  that there are only finitely many of those, therefore at some point, this list will be empty
+  in which case a fixpoint has been reached*)
 Lemma p_derivative_closure_convergence : forall (c0 c1 : Contract), exists (n:nat),
  approx_p_derivative_closure n (c0,c1) =  approx_p_derivative_closure (n+1) (c0,c1). 
 Proof. Admitted.
@@ -318,12 +1581,6 @@ Lemma well_founded_p_derivative_relation: well_founded p_derivative_relation.
 Proof. Admitted.
 
 Instance wf_p_derivative_relation : WellFounded p_derivative_relation := well_founded_p_derivative_relation.
-
-Lemma nil_i_convergence : forall (internal_nodes : list (Contract*Contract)),
-   p_derivative_closure_once (internal_nodes,[]) = (internal_nodes,[]).
-Proof. 
-intros. simpl. now rewrite <- app_nil_end.
-Qed.
 
 Lemma list_not_eq : forall (A:Type) (l0 l1 : list A) (p : A), l0++p::l1 = l0 -> False.
 Proof.
@@ -350,24 +1607,20 @@ unfold p_derivative_relation. split.
 Qed.
 Global Transparent p_derivative_closure.
 
-Definition derivative_closure (c0 c1 : Contract) := p_derivative_closure ([],[(c0,c1)]).
-Lemma in_derivative_closure : forall (c0 c1 : Contract), In (c0,c1) (derivative_closure c0 c1).
+
+Definition derivative_closure (c0 c1 : Contract) : list (Contract*Contract) := p_derivative_closure ([],[(c0,c1)]).
+
+
+(*Show lemma that all derivatives are in derivative_closure*)
+Lemma derivative_closure_is_bisimulation : forall (c0 c1 : Contract), 
+ Forall (fun (p : Contract * Contract) => nu (fst p) = nu (snd p)) (derivative_closure c0 c1) -> bisimulation (fun x y => (In (x,y) (derivative_closure c0 c1))).
 Proof. Admitted.
 
 Definition decide_contract_equivalence (c0 c1 : Contract) := 
  forallb (fun (p : Contract * Contract) => eqb (nu (fst p)) (nu (snd p)) ) (derivative_closure c0 c1).
 
-(*Forall Bisimilar c0 c1, there exists a finite_bisimulation list
-  ie, all contract equivalences can be decided by finding this list *)
-Lemma Bisimilarity_i_in_finite_bisimulation : 
- forall (c0 c1 : Contract), Bisimilarity c0 c1 -> 
-   exists l, is_finite_bisimulation l /\ In (c0,c1) l.
+Lemma Bisimilarity_reflect : forall (c0 c1 : Contract), reflect (Bisimilarity c0 c1) (decide_contract_equivalence c0 c1).
 Proof. Admitted.
-
-Lemma Bisimilarity_reflected : forall (c0 c1 : Contract), reflect (Bisimilarity c0 c1) (decide_contract_equivalence c0 c1).
-Proof. Admitted.
-
-
 
 
 
